init

process/progress.v
@@ -1,133 +1,9 @@
-From SST Require Export src.expressions process.processes process.typecheck type.global type.local process.beta process.sessions process.inversion  type.isomorphism type.projection type.proj_part type.wfgC_after_step process.subject_reduction.
+From SST Require Export src.expressions process.processes process.typecheck type.global type.local process.beta process.sessions process.inversion  type.isomorphism type.projection type.proj_part type.wfgC_after_step process.subject_reduction process.progress_helper.
 Require Import List String Datatypes ZArith Relations PeanoNat.
 Open Scope list_scope.
 From Paco Require Import paco pacotac.
 Require Import Setoid Morphisms Coq.Program.Basics.
 Require Import Coq.Init.Datatypes.
-
-Lemma pc_par5 : forall M M' M'', unfoldP (M ||| (M' ||| M'')) ((M ||| M') ||| M'').
-Proof.
-  intros.
-  apply pc_trans with (M' := (M' ||| M'') ||| M). constructor.
-  apply pc_trans with (M' := (M' ||| (M'' ||| M))). constructor.
-  apply pc_trans with (M' := (M'' ||| M) ||| M'). constructor.
-  apply pc_trans with (M' := M'' ||| (M ||| M')). constructor. constructor. 
-Qed.
-
-Lemma unf_cont_l : forall M1 M1' M2,
-  unfoldP M1 M1' -> 
-  unfoldP (M1 ||| M2) (M1' ||| M2).
-Proof.
-  intros. revert M2.
-  induction H; intros.
-  - {
-      apply pc_trans with (M' := (p <-- p_rec P) ||| (M ||| M2)). apply pc_par2.
-      apply pc_trans with (M' := (p <-- Q) ||| (M ||| M2)). constructor. easy.
-      apply pc_par5. 
-      
-    }
-  - constructor. easy.
-  - apply pc_refl.
-  - apply pc_trans with (M' := (M' ||| M2)). apply IHunfoldP1. apply IHunfoldP2.
-  - constructor.
-  - constructor.
-  - {
-      apply pc_trans with (M' := (M ||| M') ||| (M'' ||| M2)). constructor.
-      apply pc_trans with (M' := (M' ||| M) ||| (M'' ||| M2)). constructor.
-      apply pc_par5.
-    }
-  - {
-      apply pc_trans with (M' := (((M ||| M') ||| M'') ||| (M''' ||| M2))). constructor.
-      apply pc_trans with (M' := ((M ||| (M' ||| M'')) ||| (M''' ||| M2))). constructor.
-      apply pc_par5.
-    }
-Qed.
-
-Lemma unf_cont_r : forall M1 M2 M2', 
-    unfoldP M2 M2' -> 
-    unfoldP (M1 ||| M2) (M1 ||| M2').
-Proof.
-  intros.
-  apply pc_trans with (M' := M2 ||| M1). constructor.
-  apply pc_trans with (M' := M2' ||| M1). apply unf_cont_l. easy.
-  constructor.
-Qed.
-
-Lemma unf_cont : forall M1 M1' M2 M2',
-    unfoldP M1 M1' -> unfoldP M2 M2' -> 
-    unfoldP (M1 ||| M2) (M1' ||| M2').
-Proof.
-  intros.
-  apply pc_trans with (M' := (M1 ||| M2')). apply unf_cont_r. easy.
-  apply unf_cont_l. easy.
-Qed.
-
-Lemma move_forward_h : forall M,
-    forall p : string,
-    InT p M ->
-    (exists (P : process) (M' : session), unfoldP M ((p <-- P) ||| M')) \/
-    (exists P : process, unfoldP M (p <-- P)).
-Proof.
-  induction M; intros.
-  - rename H into H2. unfold InT in H2. simpl in H2. destruct H2; try easy.
-    subst. right. exists p. constructor.
-  - rename H into H2. unfold InT in *. simpl in *.
-    specialize(in_or (flattenT M1) (flattenT M2) p H2); intros.
-    destruct H.
-    - specialize(IHM1 p H). 
-      destruct IHM1.
-      - destruct H0 as (P,(M',Ha)).
-        left. exists P. exists (M' ||| M2).
-        apply pc_trans with (M' := ((p <-- P) ||| M') ||| M2). apply unf_cont_l. easy. 
-        constructor.
-      - destruct H0 as (P,Ha).
-        left. exists P. exists M2. apply unf_cont_l. easy.
-    - specialize(IHM2 p H). clear IHM1 H2.
-      destruct IHM2.
-      - destruct H0 as (P,(M',Ha)).
-        left. exists P. exists (M1 ||| M').
-        apply pc_trans with (M' := M1 ||| ((p <-- P) ||| M')). apply unf_cont_r. easy.
-        apply pc_trans with (M' := (M1 ||| (p <-- P)) ||| M'). apply pc_par5.
-        apply pc_trans with (M' := ((p <-- P) ||| M1) ||| M'). constructor. constructor.
-      - destruct H0 as (P,Ha).
-        left. exists P. exists M1.
-        apply pc_trans with (M' := M1 ||| (p <-- P)). apply unf_cont_r. easy.
-        constructor.
-Qed.
-
-Lemma move_forward : forall p M G, 
-    typ_sess M G -> 
-    isgPartsC p G -> 
-    (exists P M', unfoldP M (p <-- P ||| M')) \/ (exists P, unfoldP M (p <-- P)).
-Proof.
-  intros. inversion H. subst. clear H1 H3 H4 H.
-  specialize(H2 p H0). clear H0.
-  revert H2. revert p. clear G.
-  apply move_forward_h.
-Qed.
-
-
-Lemma part_after_unf : forall M M' p,
-    unfoldP M M' -> 
-    InT p M ->
-    InT p M'.
-Proof.
-  intros. revert H0. revert p.
-  induction H; intros; try easy.
-  - apply IHunfoldP2. apply IHunfoldP1. easy.
-  - unfold InT in *.
-    simpl in *. apply in_swap. easy.
-  - unfold InT in *. simpl in *.
-    specialize(app_assoc (flattenT M) (flattenT M') (flattenT M'')); intros.
-    replace (flattenT M ++ flattenT M' ++ flattenT M'') with ((flattenT M ++ flattenT M') ++ flattenT M'') in *. easy.
-  - unfold InT in *. simpl in *.
-    apply in_or_app. specialize(in_or ((flattenT M ++ flattenT M')) (flattenT M'') p H0); intros.
-    destruct H.
-    - left. apply in_swap. easy. right. easy.
-  - unfold InT in *. simpl in *.
-    specialize(app_assoc (flattenT M) (flattenT M') (flattenT M'')); intros.
-    replace (flattenT M ++ flattenT M' ++ flattenT M'') with ((flattenT M ++ flattenT M') ++ flattenT M'') in *. easy.
-Qed.
 
 Lemma canonical_glob_nt : forall M p q l,
     typ_sess M (gtt_send p q l) -> 
@@ -161,33 +37,6 @@ Proof.
     inversion H9; try easy.
 Qed.
 
-Lemma sub_mon : monotone2 subtype.
-Proof.
-  unfold monotone2.
-  intros.
-  induction IN; intros.
-  - constructor.
-  - constructor.
-    revert H. revert xs. induction ys; intros. constructor.
-    destruct xs; try easy.
-    simpl in *.
-    - destruct a. destruct p0. destruct o; try easy.
-      destruct p0. destruct H as (Ha,(Hb,Hc)). split. easy.
-      split. apply LE. easy. apply IHys; try easy.
-    - destruct o. destruct p0. apply IHys; try easy. 
-      apply IHys; try easy.
-  - constructor.
-    revert H. revert ys.
-    induction xs; intros.
-    - constructor.
-      destruct ys; try easy.
-      simpl in *.
-      destruct a. destruct p0. destruct o; try easy.
-      destruct p0. destruct H as (Ha,(Hb,Hc)). split. easy. split. apply LE. easy.
-      apply IHxs. easy.
-      destruct o. destruct p0. apply IHxs. easy. apply IHxs. easy.
-Qed.
-
 Lemma canonical_glob_n : forall M,
     typ_sess M gtt_end -> 
     exists M', unfoldP M M' /\ ForallT (fun _ P => P = p_inact \/ (exists e p1 p2, P = p_ite e p1 p2 /\ typ_proc nil nil (p_ite e p1 p2) ltt_end)) M'.
@@ -206,23 +55,23 @@ Proof.
       apply pc_refl.
       constructor. left. easy.
       subst.
-      specialize(_a23_bf pt l e g (p_send pt l e g) nil nil ltt_end Hb (eq_refl (p_send pt l e g))); intros.
+      specialize(inv_proc_send pt l e g (p_send pt l e g) nil nil ltt_end Hb (eq_refl (p_send pt l e g))); intros.
       destruct H1 as (S1,(T1,(Hd,(He,Hf)))). pinversion Hf.
       apply sub_mon.
       subst.
-      specialize(_a23_a p0 lis (p_recv p0 lis) nil nil ltt_end Hb (eq_refl (p_recv p0 lis))); intros.
+      specialize(inv_proc_recv p0 lis (p_recv p0 lis) nil nil ltt_end Hb (eq_refl (p_recv p0 lis))); intros.
       destruct H1 as (STT,(Hd,(He,(Hf,Hg)))). pinversion He. apply sub_mon.
     apply proj_mon.
     pinversion Ha. subst.
     inversion Hc; try easy.
     - subst. exists (s <-- p_inact). split. apply pc_refl. constructor. left. easy.
     - subst.
-      specialize(_a23_bf pt l e g (p_send pt l e g) nil nil ltt_end Hb (eq_refl (p_send pt l e g))); intros. destruct H1 as (S1,(T1,(Hd,(He,Hf)))). pinversion Hf. apply sub_mon.
+      specialize(inv_proc_send pt l e g (p_send pt l e g) nil nil ltt_end Hb (eq_refl (p_send pt l e g))); intros. destruct H1 as (S1,(T1,(Hd,(He,Hf)))). pinversion Hf. apply sub_mon.
     - subst.
-      specialize(_a23_a p0 lis (p_recv p0 lis) nil nil ltt_end Hb (eq_refl (p_recv p0 lis))); intros.
+      specialize(inv_proc_recv p0 lis (p_recv p0 lis) nil nil ltt_end Hb (eq_refl (p_recv p0 lis))); intros.
       destruct H1 as (STT,(Hd,(He,(Hf,Hg)))). pinversion He. apply sub_mon.
     - subst.
-      specialize(_a23_c (p_ite e P Q) e P Q ltt_end nil nil Hb (eq_refl (p_ite e P Q))); intros.
+      specialize(inv_proc_ite (p_ite e P Q) e P Q ltt_end nil nil Hb (eq_refl (p_ite e P Q))); intros.
       destruct H1 as (T1,(T2,(Hd,(He,(Hf,(Hg,Hh)))))).
       pinversion Hf. subst. pinversion Hg. subst.
       exists (s <-- p_ite e P Q). split. apply pc_refl.
@@ -239,7 +88,7 @@ Proof.
               P = p_ite e p1 p2 /\ typ_proc nil nil (p_ite e p1 p2) ltt_end)) M').
       {
         apply IHm; try easy.
-        - specialize(_a23_d (p_rec g) g ltt_end nil nil Hb (eq_refl (p_rec g))); intros.
+        - specialize(inv_proc_rec (p_rec g) g ltt_end nil nil Hb (eq_refl (p_rec g))); intros.
           destruct H1 as (T1,(Hd,He)). pinversion He. subst.
           specialize(_a21f g (p_rec g) ltt_end ltt_end nil nil Q); intros.
           apply H1; try easy. apply sub_mon.
@@ -255,202 +104,6 @@ Proof.
     destruct IHM2 as (M2',(Hc,Hd)). exists (M1' ||| M2'). 
     split. apply unf_cont; try easy.
     constructor; try easy.
-Qed.
-
-Lemma expr_eval_n : forall e, typ_expr nil e snat -> (exists k, stepE e (e_val (vnat k))).
-Proof.
-  induction e; intros; try easy.
-  - specialize(inv_expr_var (e_var n) n nil snat H (eq_refl (e_var n))); intros.
-    destruct H0 as (S',(Ha,Hb)). destruct n; try easy.
-  - specialize(inv_expr_vali nil (e_val v) snat v H (eq_refl (e_val v))); intros.
-    destruct H0.
-    - destruct H0 as (k,(Ha,Hb)). subst. easy.
-    - destruct H0. destruct H0 as (k,(Ha,Hb)). subst. exists k. constructor.
-    - destruct H0 as (k,(Ha,Hb)). subst. easy.
-  - specialize(inv_expr_succ nil (e_succ e) snat e H (eq_refl (e_succ e))); intros.
-    destruct H0 as (H0,H1). destruct H1. specialize(IHe H0). destruct IHe as (k,Ha). exists (k+1). constructor. easy. easy.
-  - specialize(inv_expr_neg nil (e_neg e) snat e H (eq_refl (e_neg e))); intros.
-    easy.
-  - specialize(inv_expr_not nil (e_not e) snat e H (eq_refl (e_not e))); intros.
-    destruct H0. easy.
-  - specialize(inv_expr_gt nil (e_gt e1 e2) snat e1 e2 H (eq_refl (e_gt e1 e2))); intros.
-    destruct H0 as (Ha,(Hb,Hc)). easy.
-  - specialize(inv_expr_plus nil (e_plus e1 e2) snat e1 e2 H (eq_refl (e_plus e1 e2))); intros.
-    easy.
-  - specialize(inv_expr_det nil (e_det e1 e2) snat e1 e2 H (eq_refl (e_det e1 e2))); intros.
-    destruct H0 as (k,(Ha,(Hb,Hc))). inversion Hc. subst.
-    specialize(IHe1 Ha). destruct IHe1. exists x. constructor. easy.
-Qed.
-
-Lemma expr_eval_i : forall e, typ_expr nil e sint -> (exists k, stepE e (e_val (vint k))) \/ (exists k, stepE e (e_val (vnat k))).
-Proof.
-  induction e; intros; try easy.
-  - specialize(inv_expr_var (e_var n) n nil sint H (eq_refl (e_var n))); intros.
-    destruct H0 as (S',(Ha,Hb)). destruct n; try easy.
-  - specialize(inv_expr_vali nil (e_val v) sint v H (eq_refl (e_val v))); intros.
-    destruct H0.
-    - destruct H0 as (k,(Ha,Hb)). subst. left. exists k. constructor.
-    - destruct H0. destruct H0 as (k,(Ha,Hb)). subst. right. exists k. constructor.
-    - destruct H0 as (k,(Ha,Hb)). subst. easy.
-  - specialize(inv_expr_succ nil (e_succ e) sint e H (eq_refl (e_succ e))); intros.
-    destruct H0 as (H0,H1). destruct H1. right. easy.
-    specialize(expr_eval_n e H0); intros. destruct H2 as (k,H2). 
-    right. exists (k+1). constructor. easy.
-  - specialize(inv_expr_neg nil (e_neg e) sint e H (eq_refl (e_neg e))); intros.
-    destruct H0. specialize(IHe H1).
-    destruct IHe.
-    - destruct H2 as (k,Ha). left. exists (Z.opp k). constructor. easy.
-    - destruct H2 as (k,Ha). left. exists (Z.opp (Z.of_nat k)). apply ec_neg2. easy.
-  - specialize(inv_expr_not nil (e_not e) sint e H (eq_refl (e_not e))); intros.
-    destruct H0. easy.
-  - specialize(inv_expr_gt nil (e_gt e1 e2) sint e1 e2 H (eq_refl (e_gt e1 e2))); intros.
-    destruct H0 as (Ha,(Hb,Hc)). easy.
-  - specialize(inv_expr_plus nil (e_plus e1 e2) sint e1 e2 H (eq_refl (e_plus e1 e2))); intros.
-    destruct H0 as (Ha,(Hb,Hc)). specialize(IHe1 Hb). specialize(IHe2 Hc).
-    left.
-    - destruct IHe1.
-      destruct H0 as (k,H0).
-      destruct IHe2.
-      - destruct H1 as (k1,H1). exists (Z.add k k1). constructor; try easy.
-      - destruct H1 as (k1,H1). exists (Z.add k (Z.of_nat k1)). constructor; try easy.
-    - destruct H0 as (k,H0).
-      destruct IHe2.
-      - destruct H1 as (k1,H1). exists (Z.add (Z.of_nat k) k1). constructor; try easy.
-      - destruct H1 as (k1,H1). exists (Z.add (Z.of_nat k) (Z.of_nat k1)). constructor; try easy.
-  - specialize(inv_expr_det nil (e_det e1 e2) sint e1 e2 H (eq_refl (e_det e1 e2))); intros.
-    destruct H0 as (k,(Ha,(Hb,Hc))). inversion Hc. subst.
-    - specialize(expr_eval_n e1 Ha); intros. destruct H0 as (k,Hd). right. exists k. constructor. easy.
-    - subst.
-      specialize(IHe1 Ha). destruct IHe1.
-      destruct H0. left. exists x. constructor. easy.
-      destruct H0. right. exists x. constructor. easy.
-Qed.
-
-Lemma expr_eval_b : forall e, typ_expr nil e sbool -> (stepE e (e_val (vbool true)) \/ stepE e (e_val (vbool false))).
-Proof.
-  induction e; intros; try easy.
-  - specialize(inv_expr_var (e_var n) n nil sbool H (eq_refl (e_var n))); intros.
-    destruct H0 as (S',(Ha,Hb)). destruct n; try easy.
-  - specialize(inv_expr_vali nil (e_val v) sbool v H (eq_refl (e_val v))); intros.
-    destruct H0.
-    - destruct H0 as (k,(Ha,Hb)). easy.
-    - destruct H0. destruct H0 as (k,(Ha,Hb)). subst. inversion Ha.
-    - destruct H0 as (k,(Ha,Hb)). subst. destruct k. left. apply ec_refl. right. apply ec_refl. 
-  - specialize(inv_expr_succ nil (e_succ e) sbool e H (eq_refl (e_succ e))); intros.
-    destruct H0 as (H0,H1). destruct H1. right. easy. easy.
-  - specialize(inv_expr_neg nil (e_neg e) sbool e H (eq_refl (e_neg e))); intros.
-    easy.
-  - specialize(inv_expr_not nil (e_not e) sbool e H (eq_refl (e_not e))); intros.
-    destruct H0.
-    specialize(IHe H1).
-    destruct IHe. right. constructor; try easy.
-    left. constructor; try easy.
-  - specialize(inv_expr_gt nil (e_gt e1 e2) sbool e1 e2 H (eq_refl (e_gt e1 e2))); intros.
-    destruct H0 as (Ha,(Hb,Hc)).
-    specialize(expr_eval_i e1 Hb); intros. 
-    specialize(expr_eval_i e2 Hc); intros.
-    clear Ha H IHe1 IHe2.
-    destruct H0.
-    - destruct H as (k,H).
-      destruct H1.
-      - destruct H0 as (k1,H0). 
-        specialize(Zle_or_lt k k1); intros. destruct H1. 
-        right. apply ec_gt_f3 with (m := k) (n := k1); try easy.
-        left. apply ec_gt_t3 with (m := k) (n := k1); try easy.
-      - destruct H0 as (k1,H0).
-        specialize(Zle_or_lt k (Z.of_nat k1)); intros. destruct H1. 
-        right. apply ec_gt_f2 with (m := k) (n := k1); try easy.
-        left. apply ec_gt_t2 with (m := k) (n := k1); try easy.
-    - destruct H as (k,H).
-      destruct H1.
-      - destruct H0 as (k1,H0).
-        specialize(Zle_or_lt (Z.of_nat k) k1); intros. destruct H1. 
-        right. apply ec_gt_f1 with (m := k) (n := k1); try easy.
-        left. apply ec_gt_t1 with (m := k) (n := k1); try easy.
-      - destruct H0 as (k1,H0).
-        specialize(Zle_or_lt (Z.of_nat k) (Z.of_nat k1)); intros. destruct H1. 
-        right. apply ec_gt_f0 with (m := k) (n := k1); try easy.
-        left. apply ec_gt_t0 with (m := k) (n := k1); try easy.
-  - specialize(inv_expr_plus nil (e_plus e1 e2) sbool e1 e2 H (eq_refl (e_plus e1 e2))); intros.
-    easy.
-  - specialize(inv_expr_det nil (e_det e1 e2) sbool e1 e2 H (eq_refl (e_det e1 e2))); intros.
-    destruct H0 as (k,(Ha,(Hb,Hc))). inversion Hc. subst.
-    specialize(IHe1 Ha). destruct IHe1. left. constructor. easy. right. constructor. easy.
-Qed.
-
-Lemma expr_eval_ss : forall ex S, typ_expr nil ex S -> exists v, stepE ex (e_val v).
-Proof.
-  intros.
-  destruct S. 
-  - specialize(expr_eval_b ex H); intros. destruct H0. exists (vbool true). easy. exists (vbool false). easy.
-  - specialize(expr_eval_i ex H); intros. destruct H0. destruct H0. exists (vint x). easy. destruct H0. exists (vnat x). easy.
-  - specialize(expr_eval_n ex H); intros. destruct H0. exists (vnat x). easy.
-Qed.
-
-Inductive betaPr : relation process := 
-  | betaPr_sin : forall P Q, substitutionP 0 0 0 (p_rec P) P Q -> betaPr (p_rec P) Q.
-
-Lemma guardP_break : forall P,
-    (forall n : fin, exists m : fin, guardP n m P) -> 
-    exists Q, multi betaPr P Q /\ (Q = p_inact \/ (exists e p1 p2, Q = p_ite e p1 p2) \/ (exists pt lb ex pr, Q = p_send pt lb ex pr) \/ (exists pt llp, Q = p_recv pt llp)).
-Proof.
-  intros.
-  specialize(H 1). destruct H as (m, H).
-  revert H. revert P.
-  induction m; intros.
-  - inversion H.
-    - subst. exists p_inact. split. constructor. left. easy.
-    - subst. exists (p_send pt l e g). split. constructor. right. right. left. exists pt. exists l. exists e. exists g. easy.
-    - subst. exists (p_recv p lis). split. constructor. right. right. right. exists p. exists lis. easy.
-  - inversion H. 
-    - subst. exists p_inact. split. constructor. left. easy.
-    - subst. exists (p_send pt l e g). split. constructor. right. right. left. exists pt. exists l. exists e. exists g. easy.
-    - subst. exists (p_recv p lis). split. constructor. right. right. right. exists p. exists lis. easy.
-    - subst. exists (p_ite e P0 Q). split. constructor.
-      right. left. exists e. exists P0. exists Q. easy.
-    - subst. specialize(IHm Q H3).
-      destruct IHm as (Q1,(Ha,Hb)). exists Q1. split; try easy.
-      apply multi_step with (y := Q); try easy. 
-Qed.
-
-Lemma typ_proc_after_betaPr : forall P Q Gs Gt T, 
-    multi betaPr P Q ->
-    typ_proc Gs Gt P T -> typ_proc Gs Gt Q T.
-Proof.
-  intros. revert H0. revert T Gt Gs.
-  induction H; intros.
-  - easy.
-  - apply IHmulti. clear IHmulti H0. clear z.
-    inversion H. subst.
-    specialize(_a23_d (p_rec P) P T Gs Gt H1 (eq_refl (p_rec P))); intros.
-    destruct H2 as (T0,(Ha,Hb)).
-    specialize(_a21f P (p_rec P) T0 T0 Gs Gt y); intros.
-    specialize(typable_implies_wfC H1); intros.
-    apply tc_sub with (t := T0); try easy.
-    apply H2; try easy. apply tc_mu. easy.
-Qed.
-
-Lemma betaPr_unfold_h : forall P Q1 Q Q2 p q,
-          multi betaPr P Q1 -> 
-          multi betaPr Q Q2 ->
-          unfoldP (((p <-- P) ||| (q <-- Q))) (((p <-- Q1) ||| (q <-- Q2))).
-Proof.
-  intros.
-  apply pc_trans with (M' := (p <-- Q1) ||| (q <-- Q)).
-  - apply unf_cont_l. clear H0. clear Q Q2. 
-    induction H; intros. constructor. apply pc_trans with (M' := (p <-- y)); try easy.
-    clear IHmulti H0. inversion H. subst. constructor. easy.
-  - apply unf_cont_r. clear H. clear P Q1.
-    induction H0; intros. constructor. apply pc_trans with (M' := (q <-- y)); try easy.
-    clear IHmulti H0. inversion H. subst. constructor. easy.
-Qed.
-
-Lemma betaPr_unfold : forall P Q1 Q Q2 p q M',
-          multi betaPr P Q1 -> 
-          multi betaPr Q Q2 ->
-          unfoldP (((p <-- P) ||| (q <-- Q)) ||| M') (((p <-- Q1) ||| (q <-- Q2)) ||| M').
-Proof.
-  intros. apply unf_cont_l; try easy. apply betaPr_unfold_h; try easy.
 Qed.
 
 Theorem _3_23 : forall M G, typ_sess M G -> (exists M', unfoldP M M' /\ (ForallT (fun _ P => P = p_inact) M')) \/ exists M', betaP M M'.
@@ -504,7 +157,7 @@ Proof.
         clear H0 Ha.
         assert(exists M2, betaP ((p <-- p_ite e p1 p2) ||| M1) M2).
         {
-          specialize(_a23_c (p_ite e p1 p2) e p1 p2 ltt_end nil nil Hb (eq_refl (p_ite e p1 p2))); intros.
+          specialize(inv_proc_ite (p_ite e p1 p2) e p1 p2 ltt_end nil nil Hb (eq_refl (p_ite e p1 p2))); intros.
           destruct H0 as (T1,(T2,(Ha,(Hf,(Hc,(Hd,He)))))).
           specialize(expr_eval_b e He); intros.
           destruct H0.
@@ -516,7 +169,7 @@ Proof.
         constructor.
       - assert(exists M2, betaP ((p <-- p_ite e p1 p2)) M2).
         { 
-          specialize(_a23_c (p_ite e p1 p2) e p1 p2 ltt_end nil nil Hb (eq_refl (p_ite e p1 p2))); intros.
+          specialize(inv_proc_ite (p_ite e p1 p2) e p1 p2 ltt_end nil nil Hb (eq_refl (p_ite e p1 p2))); intros.
           destruct H1 as (T1,(T2,(Hg,(Hf,(Hc,(Hd,He)))))).
           specialize(expr_eval_b e He); intros. destruct H1.
           - exists ((p <-- p1)). constructor. easy.
@@ -553,10 +206,10 @@ Proof.
           {
             clear Hh Hj.
             destruct Ho.
-            - subst. specialize(_a23_f p_inact (ltt_send q ys) nil nil H2 (eq_refl (p_inact))); intros. 
+            - subst. specialize(inv_proc_inact p_inact (ltt_send q ys) nil nil H2 (eq_refl (p_inact))); intros. 
               easy.
             - destruct H. destruct H as (e,(p1,(p2,Ha))). subst.
-              specialize(_a23_c (p_ite e p1 p2) e p1 p2 (ltt_send q ys) nil nil H2 (eq_refl (p_ite e p1 p2))); intros.
+              specialize(inv_proc_ite (p_ite e p1 p2) e p1 p2 (ltt_send q ys) nil nil H2 (eq_refl (p_ite e p1 p2))); intros.
               destruct H as (T1,(T2,(Ha,(Hb,(Hc,(Hd,He)))))).
               specialize(expr_eval_b e He); intros. 
               destruct H.
@@ -566,12 +219,12 @@ Proof.
                 apply r_struct with (M1' := ((p <-- p_ite e p1 p2) ||| ((q <-- Q2) ||| M'))) (M2' := ((p <-- p2) ||| ((q <-- Q2) ||| M'))); try easy. constructor. constructor. constructor. easy.
             - destruct H.
               destruct H as (pt,(lb,(ex,(pr,Ha)))). subst.
-              specialize(_a23_bf pt lb ex pr (p_send pt lb ex pr) nil nil (ltt_send q ys) H2 (eq_refl ((p_send pt lb ex pr)))); intros. destruct H as (S,(T1,(Ht,Hb))). clear H2. rename T1 into Tl. rename Hb into Hta. clear M P Q.
+              specialize(inv_proc_send pt lb ex pr (p_send pt lb ex pr) nil nil (ltt_send q ys) H2 (eq_refl ((p_send pt lb ex pr)))); intros. destruct H as (S,(T1,(Ht,Hb))). clear H2. rename T1 into Tl. rename Hb into Hta. clear M P Q.
               destruct Hl.
-              - subst. specialize(_a23_f p_inact (ltt_recv p ys0) nil nil H3 (eq_refl (p_inact))); intros. 
+              - subst. specialize(inv_proc_inact p_inact (ltt_recv p ys0) nil nil H3 (eq_refl (p_inact))); intros. 
                 easy.
               - destruct H. destruct H as (e,(p1,(p2,Ha))). subst. 
-                specialize(_a23_c (p_ite e p1 p2) e p1 p2 (ltt_recv p ys0) nil nil H3 (eq_refl (p_ite e p1 p2))); intros.
+                specialize(inv_proc_ite (p_ite e p1 p2) e p1 p2 (ltt_recv p ys0) nil nil H3 (eq_refl (p_ite e p1 p2))); intros.
                 destruct H as (T1,(T2,(Ha,(Hb,(Hc,(Hd,He)))))).
                 specialize(expr_eval_b e He); intros. 
                 destruct H.
@@ -586,13 +239,13 @@ Proof.
                   constructor. constructor. apply unf_cont_r. constructor.
                   constructor. easy.
               - destruct H. destruct H as (pt1,(lb1,(ex1,(pr1,Ha)))). subst.
-                specialize(_a23_bf pt1 lb1 ex1 pr1 (p_send pt1 lb1 ex1 pr1) nil nil (ltt_recv p ys0) H3 (eq_refl (p_send pt1 lb1 ex1 pr1))); intros.
+                specialize(inv_proc_send pt1 lb1 ex1 pr1 (p_send pt1 lb1 ex1 pr1) nil nil (ltt_recv p ys0) H3 (eq_refl (p_send pt1 lb1 ex1 pr1))); intros.
                 destruct H as (S1,(T1,(Ha,(Hb,Hc)))). pinversion Hc. apply sub_mon.
               - destruct H as (pt2,(llp,Ha)). subst.
                 specialize(expr_eval_ss ex S Ht); intros. destruct H as (v, Ha).
                 destruct Hta as (Hta,Htb).
                 pinversion Htb. subst.
-                specialize(_a23_a pt2 llp (p_recv pt2 llp) nil nil (ltt_recv p ys0) H3 (eq_refl (p_recv pt2 llp))); intros.
+                specialize(inv_proc_recv pt2 llp (p_recv pt2 llp) nil nil (ltt_recv p ys0) H3 (eq_refl (p_recv pt2 llp))); intros.
                 destruct H as (STT,(He,(Hb,(Hc,Hd)))).
                 pinversion Hb. subst.
                 assert(exists y, onth lb llp = Some y).
@@ -635,7 +288,7 @@ Proof.
                 constructor. constructor. constructor. easy. easy.
                 apply sub_mon. apply sub_mon.
             - destruct H as (pt,(llp,Ha)). subst.
-              specialize(_a23_a pt llp (p_recv pt llp) nil nil (ltt_send q ys) H2 (eq_refl (p_recv pt llp))); intros.
+              specialize(inv_proc_recv pt llp (p_recv pt llp) nil nil (ltt_send q ys) H2 (eq_refl (p_recv pt llp))); intros.
               destruct H as (STT,(Ha,(Hb,Hc))). pinversion Hb. apply sub_mon.
           }
           destruct H as (M1,Hta). exists M1.
@@ -672,10 +325,10 @@ Proof.
           {
             clear Hh Hj.
             destruct Ho.
-            - subst. specialize(_a23_f p_inact (ltt_send q ys) nil nil H2 (eq_refl (p_inact))); intros. 
+            - subst. specialize(inv_proc_inact p_inact (ltt_send q ys) nil nil H2 (eq_refl (p_inact))); intros. 
               easy.
             - destruct H. destruct H as (e,(p1,(p2,Ha))). subst.
-              specialize(_a23_c (p_ite e p1 p2) e p1 p2 (ltt_send q ys) nil nil H2 (eq_refl (p_ite e p1 p2))); intros.
+              specialize(inv_proc_ite (p_ite e p1 p2) e p1 p2 (ltt_send q ys) nil nil H2 (eq_refl (p_ite e p1 p2))); intros.
               destruct H as (T1,(T2,(Ha,(Hb,(Hc,(Hd,He)))))).
               specialize(expr_eval_b e He); intros. 
               destruct H.
@@ -685,12 +338,12 @@ Proof.
                 apply r_struct with (M1' := ((p <-- p_ite e p1 p2) ||| ((q <-- Q2)))) (M2' := ((p <-- p2) ||| ((q <-- Q2)))); try easy. constructor. constructor. constructor. easy.
             - destruct H.
               destruct H as (pt,(lb,(ex,(pr,Ha)))). subst.
-              specialize(_a23_bf pt lb ex pr (p_send pt lb ex pr) nil nil (ltt_send q ys) H2 (eq_refl ((p_send pt lb ex pr)))); intros. destruct H as (S,(T1,(Ht,Hb))). clear H2. rename T1 into Tl. rename Hb into Hta. clear M P Q.
+              specialize(inv_proc_send pt lb ex pr (p_send pt lb ex pr) nil nil (ltt_send q ys) H2 (eq_refl ((p_send pt lb ex pr)))); intros. destruct H as (S,(T1,(Ht,Hb))). clear H2. rename T1 into Tl. rename Hb into Hta. clear M P Q.
               destruct Hl.
-              - subst. specialize(_a23_f p_inact (ltt_recv p ys0) nil nil H3 (eq_refl (p_inact))); intros. 
+              - subst. specialize(inv_proc_inact p_inact (ltt_recv p ys0) nil nil H3 (eq_refl (p_inact))); intros. 
                 easy.
               - destruct H. destruct H as (e,(p1,(p2,Ha))). subst. 
-                specialize(_a23_c (p_ite e p1 p2) e p1 p2 (ltt_recv p ys0) nil nil H3 (eq_refl (p_ite e p1 p2))); intros.
+                specialize(inv_proc_ite (p_ite e p1 p2) e p1 p2 (ltt_recv p ys0) nil nil H3 (eq_refl (p_ite e p1 p2))); intros.
                 destruct H as (T1,(T2,(Ha,(Hb,(Hc,(Hd,He)))))).
                 specialize(expr_eval_b e He); intros. 
                 destruct H.
@@ -705,13 +358,13 @@ Proof.
                   constructor. constructor. apply unf_cont_r. constructor.
                   constructor. easy.
               - destruct H. destruct H as (pt1,(lb1,(ex1,(pr1,Ha)))). subst.
-                specialize(_a23_bf pt1 lb1 ex1 pr1 (p_send pt1 lb1 ex1 pr1) nil nil (ltt_recv p ys0) H3 (eq_refl (p_send pt1 lb1 ex1 pr1))); intros.
+                specialize(inv_proc_send pt1 lb1 ex1 pr1 (p_send pt1 lb1 ex1 pr1) nil nil (ltt_recv p ys0) H3 (eq_refl (p_send pt1 lb1 ex1 pr1))); intros.
                 destruct H as (S1,(T1,(Ha,(Hb,Hc)))). pinversion Hc. apply sub_mon.
               - destruct H as (pt2,(llp,Ha)). subst.
                 specialize(expr_eval_ss ex S Ht); intros. destruct H as (v, Ha).
                 destruct Hta as (Hta,Htb).
                 pinversion Htb. subst.
-                specialize(_a23_a pt2 llp (p_recv pt2 llp) nil nil (ltt_recv p ys0) H3 (eq_refl (p_recv pt2 llp))); intros.
+                specialize(inv_proc_recv pt2 llp (p_recv pt2 llp) nil nil (ltt_recv p ys0) H3 (eq_refl (p_recv pt2 llp))); intros.
                 destruct H as (STT,(He,(Hb,(Hc,Hd)))).
                 pinversion Hb. subst.
                 assert(exists y, onth lb llp = Some y).
@@ -754,7 +407,7 @@ Proof.
                 constructor. constructor. constructor. easy. easy.
                 apply sub_mon. apply sub_mon.
             - destruct H as (pt,(llp,Ha)). subst.
-              specialize(_a23_a pt llp (p_recv pt llp) nil nil (ltt_send q ys) H2 (eq_refl (p_recv pt llp))); intros.
+              specialize(inv_proc_recv pt llp (p_recv pt llp) nil nil (ltt_send q ys) H2 (eq_refl (p_recv pt llp))); intros.
               destruct H as (STT,(Ha,(Hb,Hc))). pinversion Hb. apply sub_mon.
           }
           destruct H as (M1,Hta). exists M1.
