process/sessions.v
@@ -1,4 +1,4 @@
-From SST Require Export src.expressions process.processes process.substitution process.inversion process.inversion_expr process.typecheck type.global type.local type.isomorphism type.projection.
+From SST Require Export src.expressions process.processes process.substitution process.inversion process.inversion_expr process.typecheck process.sessions_helper type.global type.local type.isomorphism type.projection.
 Require Import List String Datatypes ZArith Relations PeanoNat.
 Open Scope list_scope.
 Require Import Setoid Morphisms Coq.Program.Basics.
@@ -49,90 +49,6 @@ Inductive typ_sess : session -> gtt -> Prop :=
                          ForallT (fun u P => exists T, projectionC G u T /\ typ_proc nil nil P T /\ (forall n, exists m, guardP n m P)) M ->
                          typ_sess M G.
 
-
-Lemma noin_mid {A} : forall (l1 l2 : list A) a a0, ~ In a0 (l1 ++ a :: l2) -> ~ In a0 (l1 ++ l2) /\ a <> a0.
-Proof.
-  induction l1; intros; try easy.
-  simpl in *.
-  specialize(Classical_Prop.not_or_and (a = a0) (In a0 l2) H); intros.
-  easy.
-  simpl in *. 
-  specialize(Classical_Prop.not_or_and (a = a1) (In a1 (l1 ++ a0 :: l2)) H); intros.
-  destruct H0.
-  specialize(IHl1 l2 a0 a1 H1). destruct IHl1.
-  split; try easy.
-  apply Classical_Prop.and_not_or. split; try easy.
-Qed.
-
-Lemma in_mid {A} : forall (l1 l2 : list A) a pt, In pt (l1 ++ a :: l2) -> (pt = a \/ In pt (l1 ++ l2)).
-Proof.
-  induction l1; intros; try easy.
-  simpl in *. destruct H. left. easy. right. easy.
-  simpl in H. destruct H. right. left. easy.
-  specialize(IHl1 l2 a0 pt H); intros. destruct IHl1. left. easy.
-  right. right. easy.
-Qed.
-
-Lemma in_or {A} : forall (l1 l2 : list A) pt, In pt (l1 ++ l2) -> In pt l1 \/ In pt l2.
-Proof.
-  induction l1; intros; try easy.
-  right. easy.
-  simpl in H.
-  destruct H.
-  - left. constructor. easy.
-  - specialize(IHl1 l2 pt H). destruct IHl1.
-    - left. right. easy.
-    - right. easy.
-Qed.
-
-Lemma noin_swap {A} : forall (l1 l2 : list A) a, ~ In a (l1 ++ l2) -> ~ In a (l2 ++ l1).
-Proof.
-  induction l2; intros. simpl in *.
-  specialize(app_nil_r l1); intros. replace (l1 ++ nil) with l1 in *. easy.
-  specialize(noin_mid l1 l2 a a0 H); intros. destruct H0.
-  simpl in *.
-  apply Classical_Prop.and_not_or. split; try easy.
-  apply IHl2; try easy. 
-Qed.
-
-
-Lemma nodup_swap {A} : forall (l1 l2 : list A), NoDup (l1 ++ l2) -> NoDup (l2 ++ l1).
-Proof.
-  induction l2; intros. simpl in *.
-  specialize(app_nil_r l1); intros. replace (l1 ++ nil) with l1 in *. easy.
-  specialize(NoDup_remove_1 l1 l2 a H); intros.
-  specialize(NoDup_remove_2 l1 l2 a H); intros.
-  specialize(IHl2 H0).
-  constructor; try easy.
-  apply noin_swap; try easy.
-Qed.
-
-Lemma in_swap {A} : forall (l1 l2 : list A) pt, In pt (l1 ++ l2) -> In pt (l2 ++ l1).
-Proof.
-  induction l2; intros. simpl in *.
-  specialize(app_nil_r l1); intros. replace (l1 ++ nil) with l1 in *. easy.
-  specialize(in_mid l1 l2 a pt H); intros.
-  destruct H0. left. easy. right. apply IHl2; try easy.
-Qed.
-
-Lemma in_swap2 {A} : forall (l1 l2 l3 : list A) pt, In pt (l3 ++ l1 ++ l2) -> In pt (l3 ++ l2 ++ l1).
-Proof.
-  induction l3; intros. simpl in *.
-  - apply in_swap. easy.
-  - simpl in *. destruct H. left. easy.
-    specialize(IHl3 pt H). right. easy.
-Qed.
-
-Lemma nodup_swap2 {A} : forall (l1 l2 l3 : list A), NoDup (l3 ++ l1 ++ l2) -> NoDup (l3 ++ l2 ++ l1).
-Proof.
-  induction l3; intros.
-  - simpl in *. apply nodup_swap. easy.
-  - inversion H. subst. specialize(IHl3 H3). constructor; try easy.
-    unfold not in *.
-    intros. apply H2.
-    apply in_swap2. easy.
-Qed.
-
 Lemma _a22_2 : forall M M' G, typ_sess M G -> unfoldP M M' -> typ_sess M' G.
 Proof.
   intros. revert H. revert G. induction H0; intros; try easy.
@@ -141,7 +57,7 @@ Proof.
     apply t_sess; try easy. constructor; try easy. constructor; try easy.
     destruct H5. exists x. split; try easy. destruct H4. split.
     destruct H5 as (H5, H6).
-    - specialize(_a23_d (p_rec P) P x nil nil H5 (eq_refl (p_rec P))); intros.
+    - specialize(inv_proc_rec (p_rec P) P x nil nil H5 (eq_refl (p_rec P))); intros.
       destruct H7 as (T,(Ha,Hb)).
       specialize(_a21f P (p_rec P) T T nil nil Q Ha H); intros.
       specialize(typable_implies_wfC H5); intros.
@@ -157,7 +73,7 @@ Proof.
     destruct H6 as (T,(Ha,(Hb,Hc))).
     constructor; try easy.
     constructor; try easy.
-    specialize(_a23_d (p_rec P) P T nil nil Hb (eq_refl (p_rec P))); intros.
+    specialize(inv_proc_rec (p_rec P) P T nil nil Hb (eq_refl (p_rec P))); intros.
     destruct H4 as (T0,(Hd,He)).
     specialize(_a21f P (p_rec P) T0 T0 nil nil Q); intros. exists T. split. easy.
     split. specialize(typable_implies_wfC Hb); intros.
