process/sessions_helper.v
@@ -1,0 +1,89 @@
+From SST Require Export src.expressions process.processes process.substitution process.inversion process.inversion_expr process.typecheck type.global type.local type.isomorphism type.projection.
+Require Import List String Datatypes ZArith Relations PeanoNat.
+Open Scope list_scope.
+Require Import Setoid Morphisms Coq.Program.Basics.
+Require Import Coq.Init.Datatypes Coq.Logic.Classical_Prop.
+
+
+Lemma noin_mid {A} : forall (l1 l2 : list A) a a0, ~ In a0 (l1 ++ a :: l2) -> ~ In a0 (l1 ++ l2) /\ a <> a0.
+Proof.
+  induction l1; intros; try easy.
+  simpl in *.
+  specialize(Classical_Prop.not_or_and (a = a0) (In a0 l2) H); intros.
+  easy.
+  simpl in *. 
+  specialize(Classical_Prop.not_or_and (a = a1) (In a1 (l1 ++ a0 :: l2)) H); intros.
+  destruct H0.
+  specialize(IHl1 l2 a0 a1 H1). destruct IHl1.
+  split; try easy.
+  apply Classical_Prop.and_not_or. split; try easy.
+Qed.
+
+Lemma in_mid {A} : forall (l1 l2 : list A) a pt, In pt (l1 ++ a :: l2) -> (pt = a \/ In pt (l1 ++ l2)).
+Proof.
+  induction l1; intros; try easy.
+  simpl in *. destruct H. left. easy. right. easy.
+  simpl in H. destruct H. right. left. easy.
+  specialize(IHl1 l2 a0 pt H); intros. destruct IHl1. left. easy.
+  right. right. easy.
+Qed.
+
+Lemma in_or {A} : forall (l1 l2 : list A) pt, In pt (l1 ++ l2) -> In pt l1 \/ In pt l2.
+Proof.
+  induction l1; intros; try easy.
+  right. easy.
+  simpl in H.
+  destruct H.
+  - left. constructor. easy.
+  - specialize(IHl1 l2 pt H). destruct IHl1.
+    - left. right. easy.
+    - right. easy.
+Qed.
+
+Lemma noin_swap {A} : forall (l1 l2 : list A) a, ~ In a (l1 ++ l2) -> ~ In a (l2 ++ l1).
+Proof.
+  induction l2; intros. simpl in *.
+  specialize(app_nil_r l1); intros. replace (l1 ++ nil) with l1 in *. easy.
+  specialize(noin_mid l1 l2 a a0 H); intros. destruct H0.
+  simpl in *.
+  apply Classical_Prop.and_not_or. split; try easy.
+  apply IHl2; try easy. 
+Qed.
+
+
+Lemma nodup_swap {A} : forall (l1 l2 : list A), NoDup (l1 ++ l2) -> NoDup (l2 ++ l1).
+Proof.
+  induction l2; intros. simpl in *.
+  specialize(app_nil_r l1); intros. replace (l1 ++ nil) with l1 in *. easy.
+  specialize(NoDup_remove_1 l1 l2 a H); intros.
+  specialize(NoDup_remove_2 l1 l2 a H); intros.
+  specialize(IHl2 H0).
+  constructor; try easy.
+  apply noin_swap; try easy.
+Qed.
+
+Lemma in_swap {A} : forall (l1 l2 : list A) pt, In pt (l1 ++ l2) -> In pt (l2 ++ l1).
+Proof.
+  induction l2; intros. simpl in *.
+  specialize(app_nil_r l1); intros. replace (l1 ++ nil) with l1 in *. easy.
+  specialize(in_mid l1 l2 a pt H); intros.
+  destruct H0. left. easy. right. apply IHl2; try easy.
+Qed.
+
+Lemma in_swap2 {A} : forall (l1 l2 l3 : list A) pt, In pt (l3 ++ l1 ++ l2) -> In pt (l3 ++ l2 ++ l1).
+Proof.
+  induction l3; intros. simpl in *.
+  - apply in_swap. easy.
+  - simpl in *. destruct H. left. easy.
+    specialize(IHl3 pt H). right. easy.
+Qed.
+
+Lemma nodup_swap2 {A} : forall (l1 l2 l3 : list A), NoDup (l3 ++ l1 ++ l2) -> NoDup (l3 ++ l2 ++ l1).
+Proof.
+  induction l3; intros.
+  - simpl in *. apply nodup_swap. easy.
+  - inversion H. subst. specialize(IHl3 H3). constructor; try easy.
+    unfold not in *.
+    intros. apply H2.
+    apply in_swap2. easy.
+Qed.
