process/subject_reduction.v
@@ -1,463 +1,13 @@
-From SST Require Export src.expressions process.processes process.typecheck type.global type.local process.beta process.sessions process.inversion  type.isomorphism type.projection type.proj_part type.wfgC_after_step.
+From SST Require Export src.expressions process.processes process.typecheck type.global type.local process.beta process.sessions process.inversion type.isomorphism type.projection type.proj_part type.wfgC_after_step process.subject_reduction_helper.
 Require Import List String Datatypes ZArith Relations PeanoNat.
 Open Scope list_scope.
 From Paco Require Import paco pacotac.
 Require Import Setoid Morphisms Coq.Program.Basics.
 Require Import Coq.Init.Datatypes.
 
-
 Inductive multiC : relation gtt := 
   | multiC_refl : forall G, multiC G G
   | multiC_step : forall G1 G2 G3 p q n, gttstepC G1 G2 p q n -> multiC G2 G3 -> multiC G1 G3.
-  
-
-Lemma _3_21_1_helper : forall l x1 xs x4 x5 y,
-    onth l x1 = Some (x4, x5) ->
-    onth l xs = Some y ->
-    Forall2
-       (fun (u : option process) (v : option (sort * ltt)) =>
-        u = None /\ v = None \/
-        (exists (p : process) (s : sort) (t : ltt),
-           u = Some p /\ v = Some (s, t) /\ typ_proc (Some s :: nil) nil p t))
-       xs x1 ->
-    typ_proc (Some x4 :: nil) nil y x5.
-Proof.
-  induction l; intros; try easy.
-  - destruct x1. try easy. destruct xs. try easy.
-    simpl in *. subst.
-    inversion H1. subst. destruct H3. destruct H. easy.
-    destruct H. destruct H. destruct H. destruct H. destruct H0. inversion H. inversion H0. subst. easy.
-  - destruct x1; try easy. destruct xs; try easy.
-    simpl in *. apply IHl with (x1 := x1) (xs := xs); try easy.
-    inversion H1; try easy.
-Qed.
-
-Lemma noin_cat_and {A} : forall pt (l1 l2 : list A), ~ In pt (l1 ++ l2) -> ~ (In pt l1 \/ In pt l2).
-Proof.
-  induction l1; intros; try easy.
-  simpl in *. apply Classical_Prop.and_not_or. split; try easy.
-  simpl in *. specialize(Classical_Prop.not_or_and (a = pt) (In pt (l1 ++ l2)) H); intros.
-  destruct H0. 
-  apply Classical_Prop.and_not_or.
-  specialize(IHl1 l2 H1).
-  specialize(Classical_Prop.not_or_and (In pt l1) (In pt l2) IHl1); intros. destruct H2.
-  split; try easy. apply Classical_Prop.and_not_or. split; try easy.
-Qed.
-
-Lemma wfC_helper : forall l LQ SL' TL' lis,
-    onth l LQ = Some (SL', TL') -> 
-    Forall2
-       (fun (u : option (sort * local)) (v : option (sort * ltt)) =>
-        u = None /\ v = None \/
-        (exists (s : sort) (g : local) (g' : ltt),
-           u = Some (s, g) /\ v = Some (s, g') /\ upaco2 lttT bot2 g g')) lis LQ -> 
-    exists T, onth l lis = Some(SL', T) /\ lttTC T TL'.
-Proof.
-  induction l; intros.
-  - destruct LQ; try easy.
-    inversion H0. subst. clear H0 H5. simpl in H.
-    subst. destruct H4; try easy.
-    destruct H as (s,(g,(g',(Ha,(Hb,Hc))))). subst. inversion Hb. subst.
-    exists g. destruct Hc; try easy.
-  - destruct LQ ;try easy.
-    inversion H0. subst. clear H0. 
-    specialize(IHl LQ SL' TL' l0). apply IHl; try easy.
-Qed.
-
-Lemma wfC_recv :  forall [l LQ SL' TL' q],
-        wfC (ltt_recv q LQ) -> 
-        onth l LQ = Some (SL', TL') -> 
-        wfC TL'.
-Proof.  
-  intros.
-  unfold wfC in *.
-  destruct H as (T,(Ha,(Hb,Hc))).
-  specialize(guard_breakL_s2 (ltt_recv q LQ) T Hc Hb Ha); intros.
-  clear Ha Hb Hc. clear T.
-  destruct H as (T,(Hb,(Hc,(Hd,He)))).
-  destruct Hb.
-  - subst. pinversion He; try easy. apply lttT_mon.
-  - destruct H as (p0,(lis,Hf)).
-    destruct Hf. subst. pinversion He. apply lttT_mon.
-  - subst. pinversion He; try easy. subst.
-    specialize(wfC_helper l LQ SL' TL' lis H0 H1); intros.
-    destruct H as (T,(Hf,Hg)).
-    exists T. split. easy. clear Hg H1 H0 He.
-    clear TL' LQ.
-    split.
-    - inversion Hd. subst.
-      clear H1 Hd Hc. revert Hf H2. revert lis. induction l; intros; try easy.
-      - destruct lis; try easy. inversion H2. subst. clear H2 H3.
-        simpl in *. subst. destruct H1; try easy.
-        destruct H as (s,(g,(Ha,Hb))). inversion Ha. subst. easy.
-      - destruct lis; try easy. inversion H2. subst. clear H2.
-        specialize(IHl lis). apply IHl; try easy.
-    - intros. specialize(Hc (S n)).
-      destruct Hc. inversion H. subst. 
-      clear Hd H. revert Hf H3. revert lis.
-      induction l; intros; try easy.
-      - destruct lis; try easy.
-        inversion H3. subst. clear H3 H2. simpl in *. subst.
-        destruct H1; try easy. destruct H as (s,(g,(Ha,Hb))). inversion Ha. subst.
-        exists x. easy.
-      - destruct lis; try easy.
-        inversion H3. subst. clear H3.
-        specialize(IHl lis). apply IHl; try easy.
-    apply lttT_mon.
-Qed.
-
-Lemma wfC_send : forall [l LP SL TL p],
-        wfC (ltt_send p LP) -> 
-        onth l LP = Some (SL, TL) -> 
-        wfC TL.
-Proof.
-  intros.
-  unfold wfC in *.
-  destruct H as (T,(Ha,(Hb,Hc))).
-  specialize(guard_breakL_s2 (ltt_send p LP) T Hc Hb Ha); intros.
-  clear Ha Hb Hc. clear T.
-  destruct H as (T,(Hb,(Hc,(Hd,He)))).
-  destruct Hb.
-  - subst. pinversion He; try easy. apply lttT_mon.
-  - destruct H as (p0,(lis,Hf)).
-    destruct Hf. subst. pinversion He; try easy. subst.
-    specialize(wfC_helper l LP SL TL lis H0 H1); intros.
-    destruct H as (T,(Hf,Hg)).
-    exists T. split. easy. clear Hg H1 H0 He.
-    clear TL LP.
-    split.
-    - inversion Hd. subst.
-      clear H1 Hd Hc. revert Hf H2. revert lis. induction l; intros; try easy.
-      - destruct lis; try easy. inversion H2. subst. clear H2 H3.
-        simpl in *. subst. destruct H1; try easy.
-        destruct H as (s,(g,(Ha,Hb))). inversion Ha. subst. easy.
-      - destruct lis; try easy. inversion H2. subst. clear H2.
-        specialize(IHl lis). apply IHl; try easy.
-    - intros. specialize(Hc (S n)).
-      destruct Hc. inversion H. subst. 
-      clear Hd H. revert Hf H3. revert lis.
-      induction l; intros; try easy.
-      - destruct lis; try easy.
-        inversion H3. subst. clear H3 H2. simpl in *. subst.
-        destruct H1; try easy. destruct H as (s,(g,(Ha,Hb))). inversion Ha. subst.
-        exists x. easy.
-      - destruct lis; try easy.
-        inversion H3. subst. clear H3.
-        specialize(IHl lis). apply IHl; try easy.
-    apply lttT_mon.
-  - subst. pinversion He; try easy. apply lttT_mon.
-Qed.
-
-
-Lemma _3_19_3_helper : forall M p q G G' l L1 L2 S T xs y,
-    wfgC G ->
-    wfgC G' ->
-    projectionC G p (ltt_send q L1) -> 
-    subtypeC (ltt_send q (extendLis l (Datatypes.Some(S, T)))) (ltt_send q L1) ->
-    projectionC G q (ltt_recv p L2) -> 
-    onth l xs = Some y ->
-    ForallT
-  (fun (u : string) (P : process) =>
-   exists T : ltt,
-     projectionC G u T /\ typ_proc nil nil P T /\ (forall n : fin, exists m : fin, guardP n m P)) M ->
-    subtypeC (ltt_recv p xs) (ltt_recv p L2) -> 
-    gttstepC G G' p q l ->
-    ~ InT q M ->
-    ~ InT p M ->
-    ForallT
-  (fun (u : string) (P : process) =>
-   exists T : ltt,
-     projectionC G' u T /\ typ_proc nil nil P T /\ (forall n : fin, exists m : fin, guardP n m P)) M.
-Proof.
-  intro M. induction M; intros; try easy.
-  - unfold InT in *. simpl in H8. simpl in H9.
-    specialize(Classical_Prop.not_or_and (s = q) False H8); intros. destruct H10.
-    specialize(Classical_Prop.not_or_and (s = p0) False H9); intros. destruct H12.
-    clear H8 H9 H11 H13.
-    constructor.
-    inversion H5. subst. destruct H9 as [T' H9]. destruct H9.
-    specialize(projection_step_label G G' p0 q l L1 L2 H H1 H3 H7); intros.
-    destruct H11. destruct H11. destruct H11. destruct H11. destruct H11.
-    specialize(_3_19_3_helper G G' p0 q s l L1 L2 x x1 x0 x2 T'); intros.
-    assert(exists T'0 : ltt, projectionC G' s T'0 /\ T' = T'0).
-    apply H14; try easy.
-    clear H14. destruct H15. exists x3. split; try easy. destruct H14. rename x3 into Tl. subst. easy. 
-  - inversion H5. subst.
-    specialize(noin_cat_and q (flattenT M1) (flattenT M2) H8); intros.
-    specialize(noin_cat_and p (flattenT M1) (flattenT M2) H9); intros.
-    specialize(Classical_Prop.not_or_and (In q (flattenT M1)) (In q (flattenT M2)) H10); intros.
-    specialize(Classical_Prop.not_or_and (In p (flattenT M1)) (In p (flattenT M2)) H11); intros.
-    destruct H14. destruct H15.
-    unfold InT in *.
-    specialize(IHM1 p q G G' l L1 L2 S T xs y H H0 H1 H2 H3 H4 H12 H6 H7 H14 H15).
-    specialize(IHM2 p q G G' l L1 L2 S T xs y H H0 H1 H2 H3 H4 H13 H6 H7 H16 H17).
-    constructor; try easy.
-Qed.
-
-Lemma _3_21_helper : forall l xs x1 y,
-    onth l xs = Some y ->
-    Forall2
-        (fun (u : option process) (v : option (sort * ltt)) =>
-         u = None /\ v = None \/
-         (exists (p : process) (s : sort) (t : ltt),
-            u = Some p /\
-            v = Some (s, t) /\ typ_proc (Some s :: nil) nil p t)) xs x1 ->
-    exists s t, onth l x1 = Some(s,t) /\ typ_proc (Some s :: nil) nil y t.
-Proof.
-  induction l; intros.
-  - destruct xs; try easy.
-    destruct x1; try easy.
-    simpl in *.
-    inversion H0. subst. destruct H4; try easy. destruct H. destruct H. destruct H. destruct H. destruct H1. 
-    inversion H. subst.
-    exists x0. exists x2. split; try easy.
-  - destruct xs; try easy.
-    destruct x1; try easy. 
-    inversion H0. subst. apply IHl with (xs := xs); try easy.
-Qed.
-
-Lemma _3_21_helper_1 : forall [l LQ SL' TL' x x1 x0 q],
-        onth l LQ = Some (SL', TL') -> 
-        onth l x = Some (x0, x1) ->
-        subtypeC (ltt_recv q x) (ltt_recv q LQ) ->
-        subtypeC x1 TL' /\ subsort SL' x0.
-Proof.
-  intros.
-  specialize(subtype_recv_inv q x LQ H1); intros.
-  clear H1. revert H2 H0 H. revert q x0 x1 x TL' SL' LQ.
-  induction l; intros.
-  - destruct x; try easy. destruct LQ; try easy. simpl in *. subst.
-    inversion H2. subst. destruct H3; try easy. destruct H. destruct H. destruct H.
-    destruct H. destruct H. destruct H0. destruct H1. inversion H. inversion H0. subst. easy.
-  - destruct LQ; try easy. destruct x; try easy. 
-    inversion H2. subst.
-    specialize(IHl q x0 x1 x TL' SL' LQ). apply IHl; try easy.
-Qed.
-
-Lemma _3_21_helper_2 : forall [l LP SL TL LT S p],
-       subtypeC (ltt_send p (extendLis l (Some (S, LT)))) (ltt_send p LP) ->
-       onth l LP = Some (SL, TL) -> 
-       subtypeC LT TL /\ subsort S SL.
-Proof.
-  intros.
-  specialize(subtype_send_inv p (extendLis l (Some (S, LT))) LP H); intros.
-  clear H. revert H0 H1. revert LP SL TL LT S p.
-  induction l; intros.
-  - destruct LP; try easy. inversion H1. subst.
-    destruct H4; try easy. destruct H. destruct H. destruct H. destruct H. destruct H.
-    destruct H2. destruct H3. inversion H. simpl in H0. subst. inversion H2. subst.
-    easy.
-  - destruct LP; try easy. inversion H1. subst.
-    specialize(IHl LP SL TL LT S p). apply IHl; try easy.
-Qed. 
-
-Lemma _3_21_helper_3 : forall M G pt,
-        In pt (flattenT M) -> 
-        ForallT
-       (fun (u : string) (P : process) =>
-        exists T : ltt,
-          projectionC G u T /\ typ_proc nil nil P T /\ (forall n : fin, exists m : fin, guardP n m P))
-       M -> 
-       exists T : ltt, projectionC G pt T.
-Proof.
-  induction M; intros; try easy.
-  - simpl in H. destruct H; try easy. subst.
-    inversion H0. subst. destruct H1 as (T,(Ha,Hb)). exists T. easy.
-  - inversion H0. subst.
-    specialize(in_or (flattenT M1) (flattenT M2) pt H); intros.
-    destruct H1.
-    - specialize(IHM1 G pt H1 H3). apply IHM1; try easy.
-    - specialize(IHM2 G pt H1 H4). apply IHM2; try easy.
-Qed.
-
-Lemma guardP_cont_recv_n : forall l xs y q, 
-       (forall n : fin, exists m : fin, guardP n m (p_recv q xs)) -> 
-        onth l xs = Some y -> 
-        (forall n : fin, exists m : fin, guardP n m y).
-Proof.
-  induction l; intros; try easy.
-  - destruct xs; try easy.
-    simpl in H0. subst. specialize(H (Nat.succ n)).
-    destruct H. inversion H. subst.
-    inversion H3. subst. destruct H2; try easy.
-    destruct H0 as (g,(Ha,Hb)). inversion Ha. subst. exists x. easy.
-  - destruct xs; try easy.
-    specialize(IHl xs y q). apply IHl; try easy.
-    intros. specialize(H n0). destruct H.
-    inversion H. subst. exists 0. constructor.
-    subst. exists x. inversion H4. subst. constructor; try easy.
-Qed. 
-
-Inductive peq_w : process -> process -> Prop := 
-  | peq_var : forall n, peq_w (p_var n) (p_var n)
-  | peq_inact : peq_w p_inact p_inact
-  | peq_send : forall pt lb e e' p1 p2, peq_w p1 p2 -> peq_w (p_send pt lb e p1) (p_send pt lb e' p2)
-  | peq_recv : forall pt xs ys, Forall2 (fun u v => (u = None /\ v = None) \/ (exists p p', u = Some p /\ v = Some p' /\ peq_w p p')) xs ys -> peq_w (p_recv pt xs) (p_recv pt ys)
-  | peq_ite  : forall e1 p1 q1 e2 p2 q2, peq_w p1 p2 -> peq_w q1 q2 -> peq_w (p_ite e1 p1 q1) (p_ite e2 p2 q2)
-  | peq_rec : forall p1 p2, peq_w p1 p2 -> peq_w (p_rec p1) (p_rec p2).
-
-Lemma peq_after_incr : forall g p0 m n k l,
-        peq_w g p0 -> 
-        peq_w (incr_free m n k l g) (incr_free m n k l p0).
-Proof.
-  induction g using process_ind_ref; intros; try easy.
-  - inversion H. subst. constructor.
-  - inversion H. subst. constructor.
-  - inversion H. subst. constructor; try easy. apply IHg; try easy.
-  - inversion H0. subst. constructor; try easy.
-    revert H4 H. clear H0. revert llp m n k l.
-    induction ys; intros; try easy.
-    - destruct llp; try easy.
-    - destruct llp; try easy.
-      inversion H. subst. clear H. inversion H4. subst. clear H4.
-      specialize(IHys llp m n k l H7 H3). constructor; try easy. clear IHys H3 H7.
-      destruct H5.
-      - destruct H. subst. left. easy.
-      - destruct H as (p1,(p2,(Ha,(Hb,Hc)))). subst.
-        right. exists (incr_free m (S n) k l p1). exists (incr_free m (S n) k l p2). split. easy.
-        split. easy.
-        apply H2; try easy.
-  - inversion H. subst. constructor. apply IHg1; try easy. apply IHg2; try easy.
-  - inversion H. subst. constructor. apply IHg; try easy.
-Qed.
-
-Lemma peq_after_subst : forall g1 g Q m n k p0 p1,
-        substitutionP m n k g g1 Q -> 
-        peq_w g p0 -> peq_w g1 p1 ->
-        exists Q' : process, substitutionP m n k p0 p1 Q' /\ peq_w Q Q'.
-Proof.
-  induction g1 using process_ind_ref; intros.
-  - inversion H1. subst.
-    inversion H. subst.
-    - exists (incr_free 0 0 n0 k p0). split. constructor. 
-      apply peq_after_incr; try easy.
-    - subst. exists (p_var 0). split. constructor. easy. constructor.
-    - subst. exists (p_var y). split. constructor; try easy. constructor.
-    - subst. exists (p_var (S y)). split. constructor; try easy. constructor.
-  - inversion H1. subst. 
-    inversion H. subst. exists p_inact. split. constructor. constructor.
-  - inversion H1. subst.
-    inversion H. subst.
-    specialize(IHg1 g Q' m n k p0 p3 H12 H0 H7). destruct IHg1 as (q1,(Ha,Hb)).
-    exists (p_send pt lb e' q1). split. constructor; try easy. constructor; try easy.
-  - inversion H2. subst. inversion H0. subst.
-    clear H2 H0.
-    assert(exists ys3, Forall2 (fun u v => (u = None /\ v = None) \/ (exists p p', u = Some p /\ v = Some p' /\ substitutionP m n (S k) p0 p p')) ys ys3 /\ Forall2 (fun u v => (u = None /\ v = None) \/ (exists p p', u = Some p /\ v = Some p' /\ peq_w p p')) ys0 ys3).
-    {
-      revert H11 H6 H1 H.
-      revert llp g m n k p0 ys0.
-      induction ys; intros.
-      - destruct llp; try easy. destruct ys0; try easy. exists nil. easy.
-      - destruct llp; try easy. destruct ys0; try easy.
-        inversion H11. subst. clear H11. inversion H6. subst. clear H6.
-        inversion H. subst. clear H.
-        specialize(IHys llp g m n k p0 ys0 H7 H9 H1 H6).
-        clear H6 H9 H7.
-        destruct IHys as (ys3,(Ha,Hb)).
-        destruct H4.
-        - destruct H. subst. destruct H5. destruct H. subst.
-          exists (None :: ys3). split. constructor; try easy. left. easy. constructor; try easy. left. easy. 
-          destruct H as (p1,(p2,Hc)). easy.
-        - destruct H as (k1,(l1,(Hc,(Hd,He)))). subst.
-          destruct H5; try easy. destruct H as (p1,(p2,(Hf,(Hg,Hh)))). inversion Hf. subst.
-          specialize(H3 g l1 m n (S k) p0 p2 He H1 Hh).
-          destruct H3 as (q1,(Hg,Hi)).
-          exists (Some q1 :: ys3).
-          - split. constructor; try easy. right. exists p2. exists q1. easy.
-          - constructor; try easy. right. exists l1. exists q1. easy.
-    }
-    destruct H0 as (ys3,(Ha,Hb)). exists (p_recv pt ys3).
-    split. constructor; try easy. constructor; try easy. 
-  - inversion H1. subst. inversion H. subst.
-    specialize(IHg1_1 g Q1 m n k p0 p3 H12 H0 H6). destruct IHg1_1 as (q1,(Ha,Hb)).
-    specialize(IHg1_2 g Q2 m n k p0 q2 H13 H0 H7). destruct IHg1_2 as (q3,(Hc,Hd)).
-    exists (p_ite e2 q1 q3). split. constructor; try easy. constructor; try easy.
-  - inversion H1. subst. inversion H. subst.
-    specialize(IHg1 g Q' (S m) (S n) k p0 p3 H8 H0 H3).
-    destruct IHg1 as (q1,(Ha,Hb)). exists (p_rec q1).
-    split. constructor; try easy.
-    constructor; try easy.
-Qed.
-
-Lemma guardP_peq_w : forall p1 p2, 
-      peq_w p1 p2 -> 
-      (forall n : fin, exists m : fin, guardP n m p1) -> 
-      (forall n : fin, exists m : fin, guardP n m p2).
-Proof.
-  intros.
-  specialize(H0 n). destruct H0 as (m, H0). exists m.
-  revert H0 H. revert p1 p2 m.
-  induction n; intros; try easy.
-  - constructor.
-  - revert IHn H H0. revert n p1 p2.
-    induction m; intros; try easy.
-    inversion H0.
-    - subst. inversion H. subst. constructor.
-    - subst. inversion H. subst. constructor. apply IHn with (p1 := g); try easy.
-    - subst. inversion H. subst.
-      constructor. revert H5 H2 IHn. clear H0 H. revert ys. induction lis; intros; try easy.
-      - destruct ys; try easy.
-      - destruct ys; try easy. inversion H2. subst. clear H2. inversion H5. subst. clear H5.
-        specialize(IHlis ys H7 H3 IHn). constructor; try easy.
-        clear IHlis H3 H7.
-        destruct H4. left. easy.
-        destruct H as (p1,(p2,(Ha,(Hb,Hc)))). subst.
-        destruct H1; try easy. destruct H as (g1,(Hd,He)). inversion Hd. subst.
-        right. exists p2. split. easy. apply IHn with (p1 := g1); try easy.
-    assert(forall (p1 p2 : process),
-      peq_w p1 p2 -> guardP (S n) m p1 -> guardP (S n) m p2).
-    {
-      intros. specialize(IHm n p0 p3). apply IHm; try easy.
-    }
-    inversion H0. subst.
-    - inversion H. constructor.
-    - subst. inversion H. subst. constructor. apply IHn with (p1 := g); try easy.
-    - subst. inversion H. subst. constructor.
-      revert H6 H3. clear H0 H. revert ys.
-      induction lis; intros.
-      - destruct ys; try easy.
-      - destruct ys; try easy. inversion H6. subst. clear H6. inversion H3. subst. clear H3.
-        specialize(IHlis ys H7 H5). constructor; try easy.
-        destruct H4. left. easy.
-        destruct H as (p1,(p2,(Ha,(Hb,Hc)))). subst.
-        destruct H2; try easy. destruct H as (g1,(Hd,He)). inversion Hd. subst.
-        right. exists p2. split. easy.
-        apply IHn with (p1 := g1); try easy.
-    - subst. inversion H. subst.
-      constructor. apply H1 with (p1 := P); try easy. apply H1 with (p1 := Q); try easy.
-    - subst. inversion H. subst.
-      assert(exists Q', substitutionP 0 0 0 (p_rec p0) p0 Q' /\ peq_w Q Q').
-      {
-        apply peq_after_subst with (g1 := g) (g := p_rec g); try easy.
-      }
-      destruct H2 as (Q1,(Ha,Hb)).
-      apply gp_rec with (Q := Q1); try easy.
-      apply H1 with (p1 := Q); try easy.
-Qed.
-
-Lemma guardP_subst_expr : forall y v j k,
-    (forall n : fin, exists m : fin, guardP n m y) -> 
-    (forall n : fin, exists m : fin, guardP n m (subst_expr_proc y v j k)).
-Proof.
-  intros.
-  apply guardP_peq_w with (p1 := y); try easy.
-  clear H n. revert v j k.
-  induction y using process_ind_ref; intros; try easy.
-  - simpl. constructor.
-  - simpl. constructor.
-  - simpl. constructor. apply IHy; try easy.
-  - simpl. constructor.
-    revert H. revert pt v j k. induction llp; intros; try easy.
-    - inversion H. subst. clear H. specialize(IHllp pt v j k H3). constructor; try easy.
-      clear H3 IHllp.
-      destruct a.
-      - right. exists p. exists (subst_expr_proc p v (S j) (S k)). split. easy. split. easy.
-        apply H2; try easy.
-      - left. easy.
-  - simpl. constructor.
-    apply IHy1. apply IHy2.
-  - simpl. constructor. apply IHy.
-Qed.
 
 Theorem _3_21 : forall M M' G, typ_sess M G -> betaP M M' -> exists G', typ_sess M' G' /\ multiC G G'.
 Proof.
@@ -469,9 +19,9 @@ Proof.
     inversion H7. subst. clear H7. inversion H10. subst. clear H10. clear H1.
     destruct H6. destruct H1. destruct H7. destruct H6. rename x into T. rename x0 into T'.
     destruct H7 as (H7, Ht). destruct H5 as (H5, Htt).
-    - specialize(_a23_a q xs (p_recv q xs) nil nil T H5 (eq_refl (p_recv q xs))); intros. 
+    - specialize(inv_proc_recv q xs (p_recv q xs) nil nil T H5 (eq_refl (p_recv q xs))); intros. 
       destruct H8. destruct H8. destruct H10. destruct H11.
-    - specialize(_a23_bf p l e Q (p_send p l e Q) nil nil T' H7 (eq_refl (p_send p l e Q))); intros.
+    - specialize(inv_proc_send p l e Q (p_send p l e Q) nil nil T' H7 (eq_refl (p_send p l e Q))); intros.
       destruct H13. destruct H13. destruct H13. destruct H14. rename x0 into S. rename x1 into LT.
     
     specialize(_3_19_h q p l); intros.
@@ -547,7 +97,7 @@ Proof.
   (* T-COND *)
   inversion H0. subst. inversion H4. subst. clear H4. inversion H7. subst. clear H7.
   destruct H5. destruct H4. destruct H5 as (H5, Ha).
-  specialize(_a23_c (p_ite e P Q) e P Q x nil nil H5 (eq_refl (p_ite e P Q))); intros.
+  specialize(inv_proc_ite (p_ite e P Q) e P Q x nil nil H5 (eq_refl (p_ite e P Q))); intros.
   destruct H6. destruct H6. destruct H6. destruct H7. destruct H9. destruct H10. 
   exists G. split.
   apply t_sess; try easy. apply ForallT_par; try easy.
@@ -562,7 +112,7 @@ Proof.
   (* F-COND *)
   inversion H0. subst. inversion H4. subst. clear H4. inversion H7. subst. clear H7.
   destruct H5. destruct H4. destruct H5 as (H5, Ha).
-  specialize(_a23_c (p_ite e P Q) e P Q x nil nil H5 (eq_refl (p_ite e P Q))); intros.
+  specialize(inv_proc_ite (p_ite e P Q) e P Q x nil nil H5 (eq_refl (p_ite e P Q))); intros.
   destruct H6. destruct H6. destruct H6. destruct H7. destruct H9. destruct H10. 
   exists G. split.
   apply t_sess; try easy. apply ForallT_par; try easy.
@@ -579,9 +129,9 @@ Proof.
   - inversion H5. subst. clear H5. inversion H8. subst. clear H8. 
     inversion H9. subst. clear H9.
     destruct H6 as (T,(Ha,(Hb,Hc))). destruct H7 as (T1,(Hd,(He,Hf))).
-    - specialize(_a23_a q xs (p_recv q xs) nil nil T Hb (eq_refl (p_recv q xs))); intros. 
+    - specialize(inv_proc_recv q xs (p_recv q xs) nil nil T Hb (eq_refl (p_recv q xs))); intros. 
       destruct H5 as (STT,(Hg,(Hh,(Hi,Hj)))).
-    - specialize(_a23_bf p l e Q (p_send p l e Q) nil nil T1 He (eq_refl (p_send p l e Q))); intros.
+    - specialize(inv_proc_send p l e Q (p_send p l e Q) nil nil T1 He (eq_refl (p_send p l e Q))); intros.
       destruct H5 as (S,(T',(Hk,(Hl,Hm)))).
     
     specialize(_3_19_h q p l); intros.
@@ -651,7 +201,7 @@ Proof.
   (* T-COND *)
   inversion H0. subst. inversion H4. subst. clear H4.
   destruct H6. destruct H4. destruct H5 as (H5, Ha).
-  specialize(_a23_c (p_ite e P Q) e P Q x nil nil H5 (eq_refl (p_ite e P Q))); intros.
+  specialize(inv_proc_ite (p_ite e P Q) e P Q x nil nil H5 (eq_refl (p_ite e P Q))); intros.
   destruct H6. destruct H6. destruct H6. destruct H7. destruct H8. destruct H9. 
   exists G. split.
   apply t_sess; try easy. constructor. exists x.
@@ -665,7 +215,7 @@ Proof.
   (* F-COND *)
   inversion H0. subst. inversion H4. subst. clear H4.
   destruct H6. destruct H4. destruct H5 as (H5, Ha).
-  specialize(_a23_c (p_ite e P Q) e P Q x nil nil H5 (eq_refl (p_ite e P Q))); intros.
+  specialize(inv_proc_ite (p_ite e P Q) e P Q x nil nil H5 (eq_refl (p_ite e P Q))); intros.
   destruct H6. destruct H6. destruct H6. destruct H7. destruct H8. destruct H9. 
   exists G. split.
   apply t_sess; try easy. constructor. exists x.
