process/substitution_helper.v
@@ -1,0 +1,698 @@
+From mathcomp Require Import all_ssreflect.
+From SST Require Import src.expressions process.processes process.typecheck process.inversion process.inversion_expr type.global type.local type.isomorphism.
+Require Import List String Datatypes ZArith Relations PeanoNat.
+Open Scope list_scope.
+From mathcomp Require Import ssreflect.seq.
+Import ListNotations.
+From Paco Require Import paco.
+
+Fixpoint RemoveT (n : fin) (Gt : ctxT) : ctxT :=
+  match Gt with 
+    | x::xs =>
+      match n with 
+        | S m => x :: RemoveT m xs
+        | 0   => None :: xs 
+      end
+    | [] => []
+  end.
+
+Fixpoint extendT (n : fin) (T : ltt) (Gt : ctxT) : ctxT :=
+  match Gt with 
+    | x::xs =>
+      match n with 
+        | S m => x :: extendT m T xs
+        | 0   => Some T :: xs 
+      end 
+    | [] =>
+      match n with 
+        | S m => None :: extendT m T [] 
+        | 0   => [Some T]
+      end 
+  end.
+  
+Lemma onth_nil : forall n, @onth ltt n [] = None.
+Proof.
+  intros. induction n. easy. easy.
+Qed.
+
+
+Lemma remove_var : forall X n T Gt x, X <> n -> onth n (extendT X T Gt) = Some x -> onth n Gt = Some x.
+Proof.
+  intros X n T Gt. revert X T Gt. induction n; intros; try easy.
+  destruct X; try easy. destruct Gt. easy. simpl in H0. simpl. easy.
+  destruct X. destruct Gt; try easy. simpl in H0. simpl. 
+  specialize(onth_nil n); intros.
+  specialize(eq_trans (ssrfun.esym H1) H0); intros. easy.
+  specialize(Nat.succ_inj_wd_neg X n); intros. destruct H1. 
+  specialize(H1 H); intros. clear H2.
+  destruct Gt. 
+  - simpl in H0.
+    specialize(IHn X T [] x H1 H0); intros.
+    specialize(onth_nil n); intros.
+    specialize(eq_trans (ssrfun.esym H2) IHn); intros. easy.
+  - simpl in *. 
+    apply IHn with (X := X) (T := T); try easy.
+Qed.
+
+Lemma extend_extract : forall n (T : ltt) Gt, onth n (extendT n T Gt) = Some T.
+Proof.
+  intro n. induction n.
+  intros t gt. revert t. induction gt.
+  - intros. easy. intros. easy.
+  - destruct Gt; try easy. simpl.
+    - apply IHn.
+    - simpl. apply IHn.
+Qed.
+
+
+Lemma typable_implies_wtyped_helper : forall Pr STT,
+  Forall2
+       (fun (u : option process) (v : option (sort * ltt)) =>
+        u = None /\ v = None \/
+        (exists (p : process) (s : sort) (t : ltt), u = Some p /\ v = Some (s, t) /\ wtyped p)) Pr STT ->
+  Forall (fun u : option process => u = None \/ (exists k : process, u = Some k /\ wtyped k)) Pr.
+Proof.
+  intro Pr. induction Pr; intros; try easy.
+  destruct STT; try easy.
+  specialize(Forall2_cons_iff (fun (u : option process) (v : option (sort * ltt)) =>
+       u = None /\ v = None \/
+       (exists (p : process) (s : sort) (t : ltt), u = Some p /\ v = Some (s, t) /\ wtyped p)) a o Pr STT); intros.
+  destruct H0. specialize(H0 H). clear H H1. destruct H0.
+  apply Forall_cons; try easy.
+  destruct H.
+  - destruct H. subst. left. easy.
+  - destruct H. destruct H. destruct H. destruct H. destruct H1. subst.
+    right. exists x. easy.
+  apply IHPr with (STT := STT); try easy.
+Qed.
+
+Lemma typable_implies_wtyped [Gs : ctxS] [Gt : ctxT] [P : process] [T : ltt] : typ_proc Gs Gt P T -> wtyped P.
+Proof.
+  intros. induction H using typ_proc_ind_ref.
+  apply wp_inact.
+  apply wp_var.
+  apply wp_rec. easy.
+  apply wp_ite; try easy. easy.
+  apply wp_recv; try easy. 
+  - apply typable_implies_wtyped_helper with (STT := STT); try easy.
+  apply wp_send. easy.
+Qed.
+
+Lemma onth_exact {X} : forall (GtA GtB : list (option X)) T, onth (length GtA) (GtA ++ (T :: GtB)) = T.
+Proof.
+  intro GtA. induction GtA; intros; try easy.
+  simpl. apply IHGtA.
+Qed.
+
+Lemma onth_more {X} : forall (GtA GtB : list (option X)) y T, length GtA <= y -> onth y.+1 (GtA ++ (T :: GtB)) = onth y (GtA ++ GtB).
+Proof.
+  intro GtA. induction GtA; intros; try easy.
+  destruct y; try easy. apply IHGtA. easy.
+Qed.
+
+Lemma onth_less {X} : forall (GtA GtB : list (option X)) y T, y < length GtA -> length GtA <> y.+1 -> onth y.+1 (GtA ++ (T :: GtB)) = onth y.+1 (GtA ++ GtB). 
+Proof.
+  intro GtA. induction GtA; intros; try easy.
+  destruct y; try easy. destruct GtA; try easy. 
+  apply IHGtA; try easy. simpl in H0.
+  specialize(Nat.succ_inj_wd_neg (length GtA) y.+1); intros. destruct H1. apply H1; try easy. 
+Qed.
+
+Lemma onth_morec {A} : forall l Gtl Gtr n X x (tm : option A),
+      (l <= n) = true ->
+      length Gtl = l ->
+      onth (n + X)%coq_nat (Gtl ++ Gtr) = Some x ->
+      Some x = onth (n + X.+1)%coq_nat (Gtl ++ tm :: Gtr).
+Proof.
+  intro l. induction l; intros; try easy.
+  - specialize(length_zero_iff_nil Gtl); intros. destruct H2. specialize(H2 H0); intros. clear H3. subst.
+    simpl.
+    specialize(Nat.add_succ_r n X); intros. replace ((n + X.+1)%coq_nat) with ((n + X)%coq_nat.+1). simpl.
+    simpl in H1. easy.
+  - destruct n. easy.
+    destruct Gtl; try easy.
+    simpl in *.
+    apply IHl; try easy.
+    apply Nat.succ_inj. easy.
+Qed.
+
+Lemma onth_lessc {A} : forall l Gtl Gtr n x (tm : option A),
+      (l <= n) = false ->
+      length Gtl = l ->
+      onth n (Gtl ++ Gtr) = Some x ->
+      Some x = onth n (Gtl ++ tm :: Gtr).
+Proof.
+  intro l. induction l; intros; try easy.
+  destruct Gtl; try easy.
+  destruct n; try easy.
+  simpl in *.
+  apply IHl; try easy.
+  apply Nat.succ_inj. easy.
+Qed.
+
+Lemma SList_map {A} : forall (f : A -> A) lis,  
+  SList (map (fun u => match u with
+    | Some x => Some (f x)
+    | None   => None
+  end) lis) -> SList lis.
+Proof.
+  intros f lis. induction lis; intros; try easy. 
+  destruct a; try easy.
+  destruct lis; try easy.  
+  apply SList_b. apply IHlis. 
+  simpl in H.
+  specialize(SList_f (Some (f a)) (map (fun u : option A => match u with
+                                     | Some x => Some (f x)
+                                     | None => None
+                                     end) (o :: lis)) H); intros.
+  destruct H0; try easy. 
+  
+  apply SList_b. apply IHlis.
+  simpl in H.
+  easy.
+Qed.
+
+Lemma SList_map2 {A} : forall (f : A -> A) lis, SList lis -> 
+  SList (map (fun u => match u with
+    | Some x => Some (f x)
+    | None   => None
+  end) lis).
+Proof.
+  intros f lis. induction lis; intros; try easy.
+  destruct a; try easy.
+  destruct lis; try easy.
+  apply SList_b. apply IHlis.
+  easy.
+  apply SList_b. apply IHlis. easy.
+Qed.
+
+Lemma slideT_helper : forall llp Gs Gtl tm Gtr l X m k x,
+    length Gtl = l ->
+    Forall
+      (fun u : option process =>
+       match u with
+       | Some k =>
+           forall (X m l k0 : fin) (tm : option ltt) (Gs : ctxS) (Gtl Gtr : seq (option ltt)) (T : ltt),
+           typ_proc Gs (Gtl ++ Gtr) (incr_free l k0 X m k) T ->
+           length Gtl = l -> typ_proc Gs (Gtl ++ tm :: Gtr) (incr_free l k0 X.+1 m k) T
+       | None => True
+       end) llp ->
+    Forall2
+       (fun (u : option process) (v : option (sort * ltt)) =>
+        u = None /\ v = None \/
+        (exists (p : process) (s : sort) (t : ltt),
+           u = Some p /\ v = Some (s, t) /\ typ_proc (Some s :: Gs) (Gtl ++ Gtr) p t))
+       (map
+          (fun u : option process =>
+           match u with
+           | Some p' => Some (incr_free l k.+1 X m p')
+           | None => None
+           end) llp) x ->
+    Forall2
+      (fun (u : option process) (v : option (sort * ltt)) =>
+       u = None /\ v = None \/
+       (exists (p : process) (s : sort) (t : ltt),
+          u = Some p /\ v = Some (s, t) /\ typ_proc (Some s :: Gs) (Gtl ++ tm :: Gtr) p t))
+      (map
+         (fun u : option process =>
+          match u with
+          | Some p' => Some (incr_free l k.+1 X.+1 m p')
+          | None => None
+          end) llp) x.
+Proof.
+  intro llp. induction llp; intros; try easy.
+  - destruct x; try easy.
+  - destruct x; try easy.
+    simpl in *.
+    specialize(Forall2_cons_iff (fun (u : option process) (v : option (sort * ltt)) =>
+        u = None /\ v = None \/
+        (exists (p : process) (s : sort) (t : ltt),
+           u = Some p /\ v = Some (s, t) /\ typ_proc (Some s :: Gs) (Gtl ++ Gtr) p t)) (match a with
+        | Some p' => Some (incr_free l k.+1 X m p')
+        | None => None
+        end) o (map
+             (fun u : option process =>
+              match u with
+              | Some p' => Some (incr_free l k.+1 X m p')
+              | None => None
+              end) llp) x); intros. destruct H2. clear H3. specialize(H2 H1). clear H1.
+    destruct H2.
+    specialize(Forall_cons_iff (fun u : option process =>
+        match u with
+        | Some k =>
+            forall (X m l k0 : fin) (tm : option ltt) (Gs : ctxS) (Gtl Gtr : seq (option ltt)) (T : ltt),
+            typ_proc Gs (Gtl ++ Gtr) (incr_free l k0 X m k) T ->
+            length Gtl = l -> typ_proc Gs (Gtl ++ tm :: Gtr) (incr_free l k0 X.+1 m k) T
+        | None => True
+        end) a llp); intros. destruct H3. clear H4. specialize(H3 H0). clear H0. destruct H3.
+    apply Forall2_cons; try easy.
+    - destruct a; try easy. destruct H1. easy.
+      destruct H1. destruct H1. destruct H1. destruct H1. destruct H4. subst.
+      right. exists (incr_free (length Gtl) k.+1 X.+1 m p), x1, x2. split. easy. split. easy. 
+      inversion H1. subst. apply H0; try easy.
+    - destruct H1. destruct H1. subst. left. easy.
+      destruct H1. destruct H1. destruct H1. destruct H1. easy.
+    apply IHllp; try easy.
+Qed.
+
+Lemma slideTp : forall Q X m l k tm Gs Gtl Gtr T,
+typ_proc Gs (Gtl ++ Gtr) (incr_free l k X m Q) T -> length Gtl = l -> typ_proc Gs (Gtl ++ [tm] ++ Gtr) (incr_free l k X.+1 m Q) T.
+Proof.
+  intro Q.
+  induction Q using process_ind_ref; intros; try easy.
+  - simpl in *. 
+    specialize(inv_proc_var (p_var (if l <= n then (n + X)%coq_nat else n)) (if l <= n then (n + X)%coq_nat else n) T Gs (Gtl ++ Gtr) H (erefl (p_var (if l <= n then (n + X)%coq_nat else n)))); intros.
+    destruct H1. destruct H1.
+    case_eq (l <= n); intros.
+    - replace (l <= n) with true in H, H1.
+      apply tc_sub with (t := x); try easy. 
+      apply tc_var; try easy.
+      apply onth_morec with (l := l); try easy.
+      specialize(typable_implies_wfC H); intros; try easy.
+    - replace (l <= n) with false in H, H1.
+      apply tc_sub with (t := x); try easy.
+      apply tc_var; try easy.
+      apply onth_lessc with (l := l); try easy.
+      specialize(typable_implies_wfC H); intros; try easy.
+  - simpl in *. 
+    specialize(inv_proc_inact p_inact T Gs (Gtl++Gtr) H (erefl p_inact)); intros. subst. 
+    apply tc_inact.
+  - simpl in *.
+    specialize(inv_proc_send pt lb (incr_freeE k m ex) (incr_free l k X m Q) (p_send pt lb (incr_freeE k m ex) (incr_free l k X m Q)) Gs (Gtl ++ Gtr) T H (erefl (p_send pt lb (incr_freeE k m ex) (incr_free l k X m Q)))); intros.
+    destruct H1. destruct H1. destruct H1. destruct H2.
+    apply tc_sub with (t := (ltt_send pt (extendLis lb (Some (x, x0))))); try easy.
+    apply tc_send; try easy.
+    apply IHQ. easy. easy.
+    specialize(typable_implies_wfC H); intros; try easy.
+  - simpl in *.
+    specialize(inv_proc_recv pt (map
+             (fun u : option process =>
+              match u with
+              | Some p' => Some (incr_free l k.+1 X m p')
+              | None => None
+              end) llp) (p_recv pt
+          (map
+             (fun u : option process =>
+              match u with
+              | Some p' => Some (incr_free l k.+1 X m p')
+              | None => None
+              end) llp)) Gs (Gtl ++ Gtr) T H0 (erefl (p_recv pt
+          (map
+             (fun u : option process =>
+              match u with
+              | Some p' => Some (incr_free l k.+1 X m p')
+              | None => None
+              end) llp)))); intros.
+    destruct H2. destruct H2. destruct H3. destruct H4. 
+    apply tc_sub with (t := (ltt_recv pt x)); try easy. constructor.
+    specialize(Forall2_length H4); intros.
+    specialize(map_length (fun u : option process =>
+           match u with
+           | Some p' => Some (incr_free l k.+1 X m p')
+           | None => None
+           end) llp); intros.
+    specialize(eq_trans (esym H6) H7); intros. clear H6 H7.
+    apply eq_trans with (y := length llp); try easy. 
+    apply map_length; try easy.
+    apply SList_map2 with (f := (incr_free l k.+1 X.+1 m)); try easy.
+    specialize(SList_map (incr_free l k.+1 X m) llp H5); intros. easy.
+    apply slideT_helper; try easy.
+    specialize(typable_implies_wfC H0); intros; try easy.
+  - simpl in *.
+    specialize(inv_proc_ite (p_ite (incr_freeE k m e) (incr_free l k X m Q1) (incr_free l k X m Q2)) (incr_freeE k m e) (incr_free l k X m Q1) (incr_free l k X m Q2) T Gs (Gtl ++ Gtr) H (erefl (p_ite (incr_freeE k m e) (incr_free l k X m Q1) (incr_free l k X m Q2)))); intros.
+    destruct H1. destruct H1. destruct H1. destruct H2. destruct H3. destruct H4.
+    apply tc_ite; try easy.
+    apply tc_sub with (t := x); try easy.
+    apply IHQ1; try easy.
+    specialize(typable_implies_wfC H); intros; try easy.
+    apply tc_sub with (t := x0); try easy.
+    apply IHQ2; try easy.
+    specialize(typable_implies_wfC H); intros; try easy. 
+  - simpl in *. 
+    specialize(inv_proc_rec (p_rec (incr_free l.+1 k X m Q)) (incr_free l.+1 k X m Q) T Gs (Gtl++Gtr) H (erefl (p_rec (incr_free l.+1 k X m Q)))); intros.
+    destruct H1. destruct H1. 
+    specialize(IHQ X m l.+1 k tm Gs (Some x :: Gtl) Gtr x); intros.
+    specialize(cat_cons (Some x) Gtl Gtr); intros.
+    replace ((Some x :: Gtl) ++ Gtr) with (Some x :: Gtl ++ Gtr) in IHQ.
+    specialize(IHQ H1); intros. simpl in IHQ.
+    specialize(eq_S (length Gtl) l H0); intros.
+    specialize(IHQ H4). clear H0 H4.
+    apply tc_sub with (t := x); try easy.
+    apply tc_mu; try easy.
+    specialize(typable_implies_wfC H1); intros; try easy.
+    specialize(typable_implies_wfC H); intros; try easy.
+Qed.
+
+Lemma slideT : forall Q X m tm Gs Gt T,
+typ_proc Gs Gt (incr_free 0 0 X m Q) T -> typ_proc Gs (tm :: Gt) (incr_free 0 0 X.+1 m Q) T.
+Proof.
+  intros.
+  specialize(slideTp Q X m 0 0 tm Gs [] Gt T H); intros. simpl in H0.
+  apply H0; try easy.
+Qed.
+
+Lemma slideSp_e : forall k m ex x Gsl Gsr tm,
+  typ_expr (Gsl ++ Gsr) (incr_freeE k m ex) x ->
+  length Gsl = k ->
+  typ_expr (Gsl ++ tm :: Gsr) (incr_freeE k m.+1 ex) x.
+Proof. 
+  intros k m ex. revert k m. induction ex; intros; try easy.
+  - simpl in *. 
+    specialize(inv_expr_var (e_var (if k <= n then (n + m)%coq_nat else n)) (if k <= n then (n + m)%coq_nat else n) (Gsl ++ Gsr) x H (erefl (e_var (if k <= n then (n + m)%coq_nat else n)))); intros.
+    destruct H1. destruct H1.
+    apply sc_sub with (s := x0); try easy.
+    apply sc_var.
+    case_eq (k <= n); intros.
+    - replace (k <= n) with true in H1. subst.
+      apply onth_morec with (l := length Gsl); try easy.
+    - replace (k <= n) with false in H1. subst.
+      apply onth_lessc with (l := length Gsl); try easy.
+  - simpl in *. 
+    specialize(inv_expr_vali (Gsl ++ Gsr) (e_val v) x v H (erefl (e_val v))); intros.
+    destruct H1.
+    - subst. destruct H1. destruct H0. subst. apply sc_vali.
+    - subst. destruct H1. destruct H0. destruct H0. subst.
+      inversion H0. subst. apply sc_sub with (s := snat); try easy. apply sc_valn.
+      subst. apply sc_valn.
+    - subst. destruct H0. destruct H0. subst. apply sc_valb.
+  - simpl in *.
+    specialize(inv_expr_succ (Gsl ++ Gsr) (e_succ (incr_freeE k m ex)) x (incr_freeE k m ex) H (erefl (e_succ (incr_freeE k m ex)))); intros.
+    destruct H1. destruct H2.
+    - subst. apply sc_succ; try easy. apply IHex; try easy.
+    - subst. apply sc_sub with (s := snat); try easy. apply sc_succ; try easy. apply IHex; try easy.
+      apply sni.
+  - simpl in *.
+    specialize(inv_expr_neg (Gsl ++ Gsr) (e_neg (incr_freeE k m ex)) x (incr_freeE k m ex) H (erefl (e_neg (incr_freeE k m ex)))); intros.
+    destruct H1. subst. apply sc_neg. apply IHex; try easy.
+  - simpl in *.
+    specialize(inv_expr_not (Gsl ++ Gsr) (e_not (incr_freeE k m ex)) x (incr_freeE k m ex) H (erefl (e_not (incr_freeE k m ex)))); intros. 
+    destruct H1. subst. apply sc_not. apply IHex; try easy.
+  - simpl in *.
+    specialize(inv_expr_gt (Gsl ++ Gsr) (e_gt (incr_freeE k m ex1) (incr_freeE k m ex2)) x (incr_freeE k m ex1) (incr_freeE k m ex2) H (erefl (e_gt (incr_freeE k m ex1) (incr_freeE k m ex2)))); intros.
+    destruct H1. destruct H2.
+    subst. apply sc_gt. apply IHex1; try easy. apply IHex2; try easy.
+  - simpl in *.
+    specialize(inv_expr_plus (Gsl ++ Gsr) (e_plus (incr_freeE k m ex1) (incr_freeE k m ex2)) x (incr_freeE k m ex1) (incr_freeE k m ex2) H (erefl (e_plus (incr_freeE k m ex1) (incr_freeE k m ex2)))); intros.
+    destruct H1. destruct H2.
+    subst. apply sc_plus. apply IHex1; try easy. apply IHex2; try easy.
+  - simpl in *.
+    specialize(inv_expr_det (Gsl ++ Gsr) (e_det (incr_freeE k m ex1) (incr_freeE k m ex2)) x (incr_freeE k m ex1) (incr_freeE k m ex2) H (erefl (e_det (incr_freeE k m ex1) (incr_freeE k m ex2)))); intros.
+    destruct H1. destruct H1. destruct H2.
+    constructor; try easy.
+    apply IHex1; try easy.
+    apply sc_sub with (s := x0); intros; try easy.
+    apply IHex2; try easy.
+    apply sc_sub with (s := x0); intros; try easy.
+Qed.
+
+Lemma slideS_helper : forall llp l k X m x Gsl Gsr Gt tm,
+    length Gsl = k ->
+    Forall
+      (fun u : option process =>
+       match u with
+       | Some k =>
+           forall (X m l k0 : fin) (tm : option sort) (Gsl Gsr : seq (option sort)) 
+             (Gt : ctxT) (T : ltt),
+           typ_proc (Gsl ++ Gsr) Gt (incr_free l k0 X m k) T ->
+           length Gsl = k0 -> typ_proc (Gsl ++ tm :: Gsr) Gt (incr_free l k0 X m.+1 k) T
+       | None => True
+       end) llp ->
+    Forall2
+       (fun (u : option process) (v : option (sort * ltt)) =>
+        u = None /\ v = None \/
+        (exists (p : process) (s : sort) (t : ltt),
+           u = Some p /\ v = Some (s, t) /\ typ_proc (Some s :: Gsl ++ Gsr) Gt p t))
+       (map
+          (fun u : option process =>
+           match u with
+           | Some p' => Some (incr_free l k.+1 X m p')
+           | None => None
+           end) llp) x ->
+    Forall2
+      (fun (u : option process) (v : option (sort * ltt)) =>
+       u = None /\ v = None \/
+       (exists (p : process) (s : sort) (t : ltt),
+          u = Some p /\ v = Some (s, t) /\ typ_proc (Some s :: Gsl ++ tm :: Gsr) Gt p t))
+      (map
+         (fun u : option process =>
+          match u with
+          | Some p' => Some (incr_free l k.+1 X m.+1 p')
+          | None => None
+          end) llp) x.
+Proof.
+  intro llp. induction llp; intros; try easy.
+  - destruct x; try easy.
+  - destruct x; try easy.
+    specialize(Forall_cons_iff (fun u : option process =>
+        match u with
+        | Some k =>
+            forall (X m l k0 : fin) (tm : option sort) (Gsl Gsr : seq (option sort)) 
+              (Gt : ctxT) (T : ltt),
+            typ_proc (Gsl ++ Gsr) Gt (incr_free l k0 X m k) T ->
+            length Gsl = k0 -> typ_proc (Gsl ++ tm :: Gsr) Gt (incr_free l k0 X m.+1 k) T
+        | None => True
+        end) a llp); intros. destruct H2. specialize(H2 H0). clear H0 H3. destruct H2.
+    simpl in *.
+    specialize(Forall2_cons_iff (fun (u : option process) (v : option (sort * ltt)) =>
+        u = None /\ v = None \/
+        (exists (p : process) (s : sort) (t : ltt),
+           u = Some p /\ v = Some (s, t) /\ typ_proc (Some s :: Gsl ++ Gsr) Gt p t)) (match a with
+        | Some p' => Some (incr_free l k.+1 X m p')
+        | None => None
+        end) o (map
+             (fun u : option process =>
+              match u with
+              | Some p' => Some (incr_free l k.+1 X m p')
+              | None => None
+              end) llp) x); intros.
+    destruct H3. specialize(H3 H1). clear H1 H4. destruct H3.
+    apply Forall2_cons; try easy.
+    - destruct a; try easy. destruct H1. easy.
+      destruct H1. destruct H1. destruct H1. destruct H1. inversion H1. subst.
+      right. destruct H4. subst. exists (incr_free l (length Gsl).+1 X m.+1 p), x1, x2.
+      split. easy. split. easy. 
+      specialize(H0 X m l (length Gsl).+1 tm (Some x1 :: Gsl) Gsr Gt x2 H4).
+      simpl in H0. apply H0. easy.
+    - destruct H1. destruct H1. subst. left; easy.
+      destruct H1. destruct H1. destruct H1. destruct H1. easy.
+    apply IHllp; try easy.
+Qed.
+
+Lemma slideSp : forall Q X m l k tm Gsl Gsr Gt T,
+typ_proc (Gsl ++ Gsr) Gt (incr_free l k X m Q) T -> length Gsl = k -> typ_proc (Gsl ++ [tm] ++ Gsr) Gt (incr_free l k X m.+1 Q) T.
+Proof.
+  intro Q.
+  induction Q using process_ind_ref; intros; try easy.
+  - simpl in *. 
+    specialize(inv_proc_var (p_var (if l <= n then (n + X)%coq_nat else n)) (if l <= n then (n + X)%coq_nat else n) T (Gsl ++ Gsr) Gt H (erefl (p_var (if l <= n then (n + X)%coq_nat else n)))); intros.
+    destruct H1. destruct H1.
+    apply tc_sub with (t := x); try easy. 
+    apply tc_var; try easy.
+    specialize(typable_implies_wfC H); intros; try easy.
+  - simpl in *.
+    specialize(inv_proc_inact p_inact T (Gsl ++ Gsr) Gt H (erefl p_inact)); intros. subst.
+    apply tc_inact.
+  - simpl in *.
+    specialize(inv_proc_send pt lb (incr_freeE k m ex) (incr_free l k X m Q) (p_send pt lb (incr_freeE k m ex) (incr_free l k X m Q)) (Gsl ++ Gsr) Gt T H (erefl (p_send pt lb (incr_freeE k m ex) (incr_free l k X m Q) ))); intros.
+    destruct H1. destruct H1. destruct H1. destruct H2.
+    apply tc_sub with (t := (ltt_send pt (extendLis lb (Some (x, x0))))); try easy.
+    apply tc_send; try easy.
+    apply slideSp_e; try easy.
+    apply IHQ; try easy.
+    specialize(typable_implies_wfC H); intros; try easy. 
+  - simpl in *.
+    specialize(inv_proc_recv pt (map
+             (fun u : option process =>
+              match u with
+              | Some p' => Some (incr_free l k.+1 X m p')
+              | None => None
+              end) llp) (p_recv pt
+       (map
+          (fun u : option process =>
+           match u with
+           | Some p' => Some (incr_free l k.+1 X m p')
+           | None => None
+           end) llp)) (Gsl ++ Gsr) Gt T H0 (erefl (p_recv pt
+       (map
+          (fun u : option process =>
+           match u with
+           | Some p' => Some (incr_free l k.+1 X m p')
+           | None => None
+           end) llp)))); intros. 
+    destruct H2. destruct H2. destruct H3. destruct H4. 
+    apply tc_sub with (t := (ltt_recv pt x)); try easy. 
+    constructor.
+    specialize(Forall2_length H4); intros. 
+    specialize(map_length (fun u : option process =>
+           match u with
+           | Some p' => Some (incr_free l k.+1 X m p')
+           | None => None
+           end) llp); intros. 
+    specialize(eq_trans (esym H6) H7); intros.
+    apply eq_trans with (y := length llp); try easy. apply map_length. clear H2.
+    apply SList_map2; try easy.
+    specialize(SList_map (incr_free l k.+1 X m) llp H5); intros; try easy.
+    apply slideS_helper; try easy.
+    specialize(typable_implies_wfC H0); intros; try easy.
+  - simpl in *.
+    specialize(inv_proc_ite (p_ite (incr_freeE k m e) (incr_free l k X m Q1) (incr_free l k X m Q2)) (incr_freeE k m e) (incr_free l k X m Q1) (incr_free l k X m Q2) T (Gsl ++ Gsr) Gt H (erefl (p_ite (incr_freeE k m e) (incr_free l k X m Q1) (incr_free l k X m Q2)))); intros.
+    destruct H1. destruct H1. destruct H1. destruct H2. destruct H3. destruct H4.
+    apply tc_ite; try easy.
+    apply slideSp_e; try easy.
+    apply tc_sub with (t := x); try easy. apply IHQ1; try easy.
+    specialize(typable_implies_wfC H); intros; try easy.
+    apply tc_sub with (t := x0); try easy. apply IHQ2; try easy.
+    specialize(typable_implies_wfC H); intros; try easy.
+  - simpl in *.
+    specialize(inv_proc_rec (p_rec (incr_free l.+1 k X m Q)) (incr_free l.+1 k X m Q) T (Gsl ++ Gsr) Gt H (erefl (p_rec (incr_free l.+1 k X m Q)))); intros.
+    destruct H1. destruct H1. 
+    apply tc_sub with (t := x); try easy.
+    apply tc_mu. try easy.
+    apply IHQ; try easy.
+    specialize(typable_implies_wfC H1); intros; try easy.
+    specialize(typable_implies_wfC H); intros; try easy.
+Qed.
+
+Lemma slideS : forall Q X m tm Gs Gt T,
+typ_proc Gs Gt (incr_free 0 0 X m Q) T -> typ_proc (tm :: Gs) Gt (incr_free 0 0 X m.+1 Q) T.
+Proof.
+  intros.
+  specialize(slideSp Q X m 0 0 tm [] Gs Gt T H); intros. simpl in H0.
+  apply H0; try easy.
+Qed.
+
+Lemma _a21_helper_1 : forall llp ys (GtA : list (option ltt)) m n Q,
+      SList llp ->      
+      Forall2
+        (fun u v : option process =>
+         u = None /\ v = None \/
+         (exists k l : process, u = Some k /\ v = Some l /\ substitutionP (length GtA) m n.+1 Q k l))
+        llp ys -> 
+      SList ys.
+Proof.
+  intro llp. induction llp; intros; try easy.
+  inversion H0. subst. clear H0.
+  destruct H3. destruct H0. subst. apply SList_b. 
+  - apply IHllp with (GtA := GtA) (m := m) (n := n) (Q := Q); try easy.
+  - destruct H0. destruct H0. destruct H0. destruct H1. subst.
+    specialize(SList_f (Some x) llp H); intros.
+    destruct H0. apply SList_b. apply IHllp with (GtA := GtA) (m := m) (n := n) (Q := Q); try easy.
+    destruct H0. subst. inversion H5. subst. easy.
+Qed.
+
+Lemma _a21_recv_helper : forall llp Q Gs GtA GtB m n T ys x,
+  wtyped Q ->
+  typ_proc Gs (GtA ++ GtB) (incr_free 0 0 m n Q) T ->
+  Forall
+      (fun u : option process =>
+       match u with
+       | Some k =>
+           forall (Q : process) (T T' : ltt) (Gs : ctxS) (GtA GtB : seq (option ltt)) 
+             (X : fin) (Q' : process) (m n : fin),
+           wtyped Q ->
+           typ_proc Gs (GtA ++ Some T :: GtB) k T' ->
+           length GtA = X ->
+           substitutionP X m n Q k Q' ->
+           typ_proc Gs (GtA ++ GtB) (incr_free 0 0 m n Q) T -> typ_proc Gs (GtA ++ GtB) Q' T'
+       | None => True
+       end) llp ->
+  Forall2
+        (fun u v : option process =>
+         u = None /\ v = None \/
+         (exists k l : process, u = Some k /\ v = Some l /\ substitutionP (length GtA) m n.+1 Q k l))
+        llp ys ->
+  Forall2
+       (fun (u : option process) (v : option (sort * ltt)) =>
+        u = None /\ v = None \/
+        (exists (p : process) (s : sort) (t : ltt),
+           u = Some p /\ v = Some (s, t) /\ typ_proc (Some s :: Gs) (GtA ++ Some T :: GtB) p t)) llp x ->
+  Forall2
+  (fun (u : option process) (v : option (sort * ltt)) =>
+   u = None /\ v = None \/
+   (exists (p : process) (s : sort) (t : ltt),
+      u = Some p /\ v = Some (s, t) /\ typ_proc (Some s :: Gs) (GtA ++ GtB) p t)) ys x.
+Proof.
+  intro llp. induction llp; intros; try easy.
+  inversion H2. subst. inversion H3. subst. easy.
+  inversion H2. subst. inversion H3. subst. clear H2 H3.
+  constructor; try easy.
+  - destruct H6. destruct H2. subst.
+    left. destruct H7; try easy. destruct H2. destruct H2. destruct H2. easy.
+    destruct H2. destruct H2. destruct H2. destruct H3. subst.
+    destruct H7; try easy. destruct H2. destruct H2. destruct H2. destruct H2. destruct H3. inversion H2. subst.
+    right. exists x0. exists x2. exists x3. split; try easy. split; try easy.
+    inversion H1. subst. 
+    specialize(H7 Q T x3 (Some x2 :: Gs) GtA GtB (length GtA) x0 m n.+1). 
+    apply H7; try easy.
+    apply slideS; try easy.
+  - inversion H1. subst. clear H1 H6 H7 H4.
+    apply IHllp with (Q := Q) (m := m) (n := n) (T := T); try easy.
+Qed.
+
+Lemma trivial_incrE : forall n ex, (incr_freeE n 0 ex) = ex.
+Proof.
+  intros n ex. induction ex; intros; try easy.
+  - simpl. destruct (n <= n0); try easy.
+    specialize(Nat.add_0_r n0); intros. replace (n0 + 0)%coq_nat with n0. easy.
+  - simpl. replace (incr_freeE n 0 ex) with ex. easy.
+  - simpl. replace (incr_freeE n 0 ex) with ex. easy.
+  - simpl. replace (incr_freeE n 0 ex) with ex. easy.
+  - simpl. replace (incr_freeE n 0 ex1) with ex1. replace (incr_freeE n 0 ex2) with ex2. easy.
+  - simpl. replace (incr_freeE n 0 ex1) with ex1. replace (incr_freeE n 0 ex2) with ex2. easy.
+  - simpl. replace (incr_freeE n 0 ex1) with ex1. replace (incr_freeE n 0 ex2) with ex2. easy.
+Qed.
+
+Lemma trivial_incr : forall m n Q, (incr_free m n 0 0 Q) = Q.
+Proof.
+  intros. revert m n. induction Q using process_ind_ref; intros; simpl; try easy. 
+  - destruct (m <= n); try easy.
+    specialize(Nat.add_0_r n); intros. replace (n + 0)%coq_nat with n; easy.
+  - specialize(trivial_incrE n ex); intros.
+    specialize(IHQ m n); intros.
+    replace (incr_freeE n 0 ex) with ex. replace (incr_free m n 0 0 Q) with Q. easy.
+  - assert (map (fun u => match u with 
+        | Some u => Some (incr_free m n.+1 0 0 u)
+        | None   => None
+      end) llp = llp).
+    {
+      induction llp. easy. simpl in *.
+      specialize(Forall_cons_iff (fun u : option process =>
+       match u with
+       | Some k => forall m n : fin, incr_free m n 0 0 k = k
+       | None => True
+       end) a llp); intros.
+      destruct H0. specialize(H0 H); intros. clear H1 H. destruct H0.
+      specialize(IHllp H0); intros.
+      simpl.
+      destruct a; try easy. 
+      specialize(H m n.+1). replace (incr_free m n.+1 0 0 p) with p. 
+      replace (map
+     (fun u : option process =>
+      match u with
+      | Some u0 => Some (incr_free m n.+1 0 0 u0)
+      | None => None
+      end) llp) with llp. easy.
+      replace (map
+     (fun u : option process =>
+      match u with
+      | Some u0 => Some (incr_free m n.+1 0 0 u0)
+      | None => None
+      end) llp) with llp. easy.
+    }
+    replace (List.map (fun u : option process =>
+        match u with
+        | Some p' => Some (incr_free m n.+1 0 0 p')
+        | None => None
+        end) llp) with llp. easy.
+  - specialize(trivial_incrE n e); intros. 
+    specialize(IHQ1 m n); intros. specialize(IHQ2 m n); intros.
+    replace (incr_freeE n 0 e) with e.
+    replace (incr_free m n 0 0 Q1) with Q1. 
+    replace (incr_free m n 0 0 Q2) with Q2.
+    easy.
+  - specialize(IHQ m.+1 n); intros. 
+    replace (incr_free m.+1 n 0 0 Q) with Q. easy.
+Qed.
+
+
+
